#209 Nammes for everyone, dom lemmas for component and all component instances

abp/ABPComponent.thy
@@ -3,7 +3,7 @@
  * This file was generated from ABP.maa and will be overridden when changed. To change
  * permanently, consider changing the model itself.
  *
- * Generated on Oct 2, 2018 7:11:57 PM by isartransformer 1.0.0
+ * Generated on Oct 2, 2018 7:49:39 PM by isartransformer 1.0.0
  *)
 theory ABPComponent
   imports SenderAutomaton MediumAutomaton ReceiverAutomaton spec.SPS spec.USpec_UFunComp
@@ -11,9 +11,9 @@ theory ABPComponent
 begin
 
 
-section ‹Datatype definition›
+section \<open>Datatype definition\<close>
 
-datatype ('e::countable) abpMessage = DoNotUse_65e4c1937d484f20baf2707bdccbfc49_ABPE "'e" | DoNotUse_65e4c1937d484f20baf2707bdccbfc49_ABPBool "bool" | DoNotUse_65e4c1937d484f20baf2707bdccbfc49_ABPPair_E_Bool "('e×bool)"
+datatype ('e::countable) abpMessage = ABPE "'e" | ABPBool "bool" | ABPPair_E_Bool "('e\<times>bool)"
 
 instance abpMessage :: (countable) countable
   apply(intro_classes)
@@ -21,682 +21,682 @@ instance abpMessage :: (countable) countable
 
 instantiation abpMessage :: (countable) message
 begin
-  fun ctype_abpMessage :: "channel ⇒ ('e::countable) abpMessage set" where
+  fun ctype_abpMessage :: "channel \<Rightarrow> ('e::countable) abpMessage set" where
   "ctype_abpMessage c = (
-    if c = 𝒞 ''DoNotUse_65e4c1937d484f20baf2707bdccbfc49_receiver_o__o'' then range DoNotUse_65e4c1937d484f20baf2707bdccbfc49_ABPE else
-    if c = 𝒞 ''DoNotUse_65e4c1937d484f20baf2707bdccbfc49_i__sender_i'' then range DoNotUse_65e4c1937d484f20baf2707bdccbfc49_ABPE else
-    if c = 𝒞 ''DoNotUse_65e4c1937d484f20baf2707bdccbfc49_sender_ds__mediumSr_ar'' then range DoNotUse_65e4c1937d484f20baf2707bdccbfc49_ABPPair_E_Bool else
-    if c = 𝒞 ''DoNotUse_65e4c1937d484f20baf2707bdccbfc49_mediumSr_as__receiver_dr'' then range DoNotUse_65e4c1937d484f20baf2707bdccbfc49_ABPPair_E_Bool else
-    if c = 𝒞 ''DoNotUse_65e4c1937d484f20baf2707bdccbfc49_receiver_ar__mediumRs_ar'' then range DoNotUse_65e4c1937d484f20baf2707bdccbfc49_ABPBool else
-    if c = 𝒞 ''DoNotUse_65e4c1937d484f20baf2707bdccbfc49_mediumRs_as__sender_as'' then range DoNotUse_65e4c1937d484f20baf2707bdccbfc49_ABPBool else
+    if c = \<C> ''receiver_o__o'' then range ABPE else
+    if c = \<C> ''i__sender_i'' then range ABPE else
+    if c = \<C> ''sender_ds__mediumSr_ar'' then range ABPPair_E_Bool else
+    if c = \<C> ''mediumSr_as__receiver_dr'' then range ABPPair_E_Bool else
+    if c = \<C> ''receiver_ar__mediumRs_ar'' then range ABPBool else
+    if c = \<C> ''mediumRs_as__sender_as'' then range ABPBool else
     undefined)"
   instance
     by(intro_classes)
 end
 
 
-section ‹Domain and range›
+section \<open>Domain and range\<close>
 
 definition aBPDom :: "channel set" where
-"aBPDom = {𝒞 ''DoNotUse_65e4c1937d484f20baf2707bdccbfc49_i__sender_i''}"
+"aBPDom = {\<C> ''i__sender_i''}"
 
 definition aBPRan :: "channel set" where
-"aBPRan = {𝒞 ''DoNotUse_65e4c1937d484f20baf2707bdccbfc49_receiver_o__o''}"
+"aBPRan = {\<C> ''receiver_o__o''}"
 
 
-subsection ‹sender›
+subsection \<open>sender\<close>
 
 definition aBPSenderDom :: "channel set" where
-"aBPSenderDom = {𝒞 ''DoNotUse_65e4c1937d484f20baf2707bdccbfc49_mediumRs_as__sender_as'', 𝒞 ''DoNotUse_65e4c1937d484f20baf2707bdccbfc49_i__sender_i''}"
+"aBPSenderDom = {\<C> ''mediumRs_as__sender_as'', \<C> ''i__sender_i''}"
 
 definition aBPSenderRan :: "channel set" where
-"aBPSenderRan = {𝒞 ''DoNotUse_65e4c1937d484f20baf2707bdccbfc49_sender_ds__mediumSr_ar''}"
+"aBPSenderRan = {\<C> ''sender_ds__mediumSr_ar''}"
 
 
-subsection ‹mediumSr›
+subsection \<open>mediumSr\<close>
 
 definition aBPMediumSrDom :: "channel set" where
-"aBPMediumSrDom = {𝒞 ''DoNotUse_65e4c1937d484f20baf2707bdccbfc49_sender_ds__mediumSr_ar''}"
+"aBPMediumSrDom = {\<C> ''sender_ds__mediumSr_ar''}"
 
 definition aBPMediumSrRan :: "channel set" where
-"aBPMediumSrRan = {𝒞 ''DoNotUse_65e4c1937d484f20baf2707bdccbfc49_mediumSr_as__receiver_dr''}"
+"aBPMediumSrRan = {\<C> ''mediumSr_as__receiver_dr''}"
 
 
-subsection ‹receiver›
+subsection \<open>receiver\<close>
 
 definition aBPReceiverDom :: "channel set" where
-"aBPReceiverDom = {𝒞 ''DoNotUse_65e4c1937d484f20baf2707bdccbfc49_mediumSr_as__receiver_dr''}"
+"aBPReceiverDom = {\<C> ''mediumSr_as__receiver_dr''}"
 
 definition aBPReceiverRan :: "channel set" where
-"aBPReceiverRan = {𝒞 ''DoNotUse_65e4c1937d484f20baf2707bdccbfc49_receiver_ar__mediumRs_ar'', 𝒞 ''DoNotUse_65e4c1937d484f20baf2707bdccbfc49_receiver_o__o''}"
+"aBPReceiverRan = {\<C> ''receiver_ar__mediumRs_ar'', \<C> ''receiver_o__o''}"
 
 
-subsection ‹mediumRs›
+subsection \<open>mediumRs\<close>
 
 definition aBPMediumRsDom :: "channel set" where
-"aBPMediumRsDom = {𝒞 ''DoNotUse_65e4c1937d484f20baf2707bdccbfc49_receiver_ar__mediumRs_ar''}"
+"aBPMediumRsDom = {\<C> ''receiver_ar__mediumRs_ar''}"
 
 definition aBPMediumRsRan :: "channel set" where
-"aBPMediumRsRan = {𝒞 ''DoNotUse_65e4c1937d484f20baf2707bdccbfc49_mediumRs_as__sender_as''}"
+"aBPMediumRsRan = {\<C> ''mediumRs_as__sender_as''}"
 
 
-section ‹Helpers to create a bundle from a single raw element›
+section \<open>Helpers to create a bundle from a single raw element\<close>
 
 (* Do not use this, use aBPReceiverElemOut_ar_o or aBPElemOut_o instead *)
-lift_definition aBPElem_raw_receiver_o__o :: "'e ⇒ ('e::countable) abpMessage tsyn sbElem" is
-"λx. [𝒞 ''DoNotUse_65e4c1937d484f20baf2707bdccbfc49_receiver_o__o'' ↦ Msg (DoNotUse_65e4c1937d484f20baf2707bdccbfc49_ABPE x)]"
+lift_definition aBPElem_raw_receiver_o__o :: "'e \<Rightarrow> ('e::countable) abpMessage tsyn sbElem" is
+"\<lambda>x. [\<C> ''receiver_o__o'' \<mapsto> Msg (ABPE x)]"
   unfolding sbElemWell_def
   unfolding usclOkay_stream_def
   unfolding ctype_tsyn_def
   by simp
 
 (* Do not use this, use aBPElemIn_i or aBPSenderElemIn_as_i instead *)
-lift_definition aBPElem_raw_i__sender_i :: "'e ⇒ ('e::countable) abpMessage tsyn sbElem" is
-"λx. [𝒞 ''DoNotUse_65e4c1937d484f20baf2707bdccbfc49_i__sender_i'' ↦ Msg (DoNotUse_65e4c1937d484f20baf2707bdccbfc49_ABPE x)]"
+lift_definition aBPElem_raw_i__sender_i :: "'e \<Rightarrow> ('e::countable) abpMessage tsyn sbElem" is
+"\<lambda>x. [\<C> ''i__sender_i'' \<mapsto> Msg (ABPE x)]"
   unfolding sbElemWell_def
   unfolding usclOkay_stream_def
   unfolding ctype_tsyn_def
   by simp
 
 (* Do not use this, use aBPSenderElemOut_ds or aBPMediumSrElemIn_ar instead *)
-lift_definition aBPElem_raw_sender_ds__mediumSr_ar :: "('e×bool) ⇒ ('e::countable) abpMessage tsyn sbElem" is
-"λx. [𝒞 ''DoNotUse_65e4c1937d484f20baf2707bdccbfc49_sender_ds__mediumSr_ar'' ↦ Msg (DoNotUse_65e4c1937d484f20baf2707bdccbfc49_ABPPair_E_Bool x)]"
+lift_definition aBPElem_raw_sender_ds__mediumSr_ar :: "('e\<times>bool) \<Rightarrow> ('e::countable) abpMessage tsyn sbElem" is
+"\<lambda>x. [\<C> ''sender_ds__mediumSr_ar'' \<mapsto> Msg (ABPPair_E_Bool x)]"
   unfolding sbElemWell_def
   unfolding usclOkay_stream_def
   unfolding ctype_tsyn_def
   by simp
 
 (* Do not use this, use aBPMediumSrElemOut_as or aBPReceiverElemIn_dr instead *)
-lift_definition aBPElem_raw_mediumSr_as__receiver_dr :: "('e×bool) ⇒ ('e::countable) abpMessage tsyn sbElem" is
-"λx. [𝒞 ''DoNotUse_65e4c1937d484f20baf2707bdccbfc49_mediumSr_as__receiver_dr'' ↦ Msg (DoNotUse_65e4c1937d484f20baf2707bdccbfc49_ABPPair_E_Bool x)]"
+lift_definition aBPElem_raw_mediumSr_as__receiver_dr :: "('e\<times>bool) \<Rightarrow> ('e::countable) abpMessage tsyn sbElem" is
+"\<lambda>x. [\<C> ''mediumSr_as__receiver_dr'' \<mapsto> Msg (ABPPair_E_Bool x)]"
   unfolding sbElemWell_def
   unfolding usclOkay_stream_def
   unfolding ctype_tsyn_def
   by simp
 
 (* Do not use this, use aBPReceiverElemOut_ar_o or aBPMediumRsElemIn_ar instead *)
-lift_definition aBPElem_raw_receiver_ar__mediumRs_ar :: "bool ⇒ ('e::countable) abpMessage tsyn sbElem" is
-"λx. [𝒞 ''DoNotUse_65e4c1937d484f20baf2707bdccbfc49_receiver_ar__mediumRs_ar'' ↦ Msg (DoNotUse_65e4c1937d484f20baf2707bdccbfc49_ABPBool x)]"
+lift_definition aBPElem_raw_receiver_ar__mediumRs_ar :: "bool \<Rightarrow> ('e::countable) abpMessage tsyn sbElem" is
+"\<lambda>x. [\<C> ''receiver_ar__mediumRs_ar'' \<mapsto> Msg (ABPBool x)]"
   unfolding sbElemWell_def
   unfolding usclOkay_stream_def
   unfolding ctype_tsyn_def
   by simp
 
 (* Do not use this, use aBPMediumRsElemOut_as or aBPSenderElemIn_as_i instead *)
-lift_definition aBPElem_raw_mediumRs_as__sender_as :: "bool ⇒ ('e::countable) abpMessage tsyn sbElem" is
-"λx. [𝒞 ''DoNotUse_65e4c1937d484f20baf2707bdccbfc49_mediumRs_as__sender_as'' ↦ Msg (DoNotUse_65e4c1937d484f20baf2707bdccbfc49_ABPBool x)]"
+lift_definition aBPElem_raw_mediumRs_as__sender_as :: "bool \<Rightarrow> ('e::countable) abpMessage tsyn sbElem" is
+"\<lambda>x. [\<C> ''mediumRs_as__sender_as'' \<mapsto> Msg (ABPBool x)]"
   unfolding sbElemWell_def
   unfolding usclOkay_stream_def
   unfolding ctype_tsyn_def
   by simp
 
 
-section ‹Helpers to create a bundle from a single tsyn element›
+section \<open>Helpers to create a bundle from a single tsyn element\<close>
 
 (* Do not use this, use aBPReceiverElemOut_ar_o or aBPElemOut_o instead *)
-fun aBPElem_receiver_o__o :: "'e tsyn ⇒ ('e::countable) abpMessage tsyn sbElem" where
+fun aBPElem_receiver_o__o :: "'e tsyn \<Rightarrow> ('e::countable) abpMessage tsyn sbElem" where
 "aBPElem_receiver_o__o (Msg receiver_port_o__port_o) = aBPElem_raw_receiver_o__o receiver_port_o__port_o" |
-"aBPElem_receiver_o__o null = sbeNull {𝒞 ''DoNotUse_65e4c1937d484f20baf2707bdccbfc49_receiver_o__o''}"
+"aBPElem_receiver_o__o null = sbeNull {\<C> ''receiver_o__o''}"
 
 declare aBPElem_receiver_o__o.simps[simp del]
 
 (* Do not use this, use aBPReceiverOut_ar_o or aBPOut_o instead *)
-definition aBP_receiver_o__o :: "'e tsyn ⇒ ('e::countable) abpMessage tsyn SB" where
+definition aBP_receiver_o__o :: "'e tsyn \<Rightarrow> ('e::countable) abpMessage tsyn SB" where
 "aBP_receiver_o__o receiver_port_o__port_o = sbe2SB (aBPElem_receiver_o__o receiver_port_o__port_o)"
 
 (* Do not use this, use aBPElemIn_i or aBPSenderElemIn_as_i instead *)
-fun aBPElem_i__sender_i :: "'e tsyn ⇒ ('e::countable) abpMessage tsyn sbElem" where
+fun aBPElem_i__sender_i :: "'e tsyn \<Rightarrow> ('e::countable) abpMessage tsyn sbElem" where
 "aBPElem_i__sender_i (Msg port_i__sender_port_i) = aBPElem_raw_i__sender_i port_i__sender_port_i" |
-"aBPElem_i__sender_i null = sbeNull {𝒞 ''DoNotUse_65e4c1937d484f20baf2707bdccbfc49_i__sender_i''}"
+"aBPElem_i__sender_i null = sbeNull {\<C> ''i__sender_i''}"
 
 declare aBPElem_i__sender_i.simps[simp del]
 
 (* Do not use this, use aBPIn_i or aBPSenderIn_as_i instead *)
-definition aBP_i__sender_i :: "'e tsyn ⇒ ('e::countable) abpMessage tsyn SB" where
+definition aBP_i__sender_i :: "'e tsyn \<Rightarrow> ('e::countable) abpMessage tsyn SB" where
 "aBP_i__sender_i port_i__sender_port_i = sbe2SB (aBPElem_i__sender_i port_i__sender_port_i)"
 
 (* Do not use this, use aBPSenderElemOut_ds or aBPMediumSrElemIn_ar instead *)
-fun aBPElem_sender_ds__mediumSr_ar :: "('e×bool) tsyn ⇒ ('e::countable) abpMessage tsyn sbElem" where
+fun aBPElem_sender_ds__mediumSr_ar :: "('e\<times>bool) tsyn \<Rightarrow> ('e::countable) abpMessage tsyn sbElem" where
 "aBPElem_sender_ds__mediumSr_ar (Msg sender_port_ds__mediumSr_port_ar) = aBPElem_raw_sender_ds__mediumSr_ar sender_port_ds__mediumSr_port_ar" |
-"aBPElem_sender_ds__mediumSr_ar null = sbeNull {𝒞 ''DoNotUse_65e4c1937d484f20baf2707bdccbfc49_sender_ds__mediumSr_ar''}"
+"aBPElem_sender_ds__mediumSr_ar null = sbeNull {\<C> ''sender_ds__mediumSr_ar''}"
 
 declare aBPElem_sender_ds__mediumSr_ar.simps[simp del]
 
 (* Do not use this, use aBPSenderOut_ds or aBPMediumSrIn_ar instead *)
-definition aBP_sender_ds__mediumSr_ar :: "('e×bool) tsyn ⇒ ('e::countable) abpMessage tsyn SB" where
+definition aBP_sender_ds__mediumSr_ar :: "('e\<times>bool) tsyn \<Rightarrow> ('e::countable) abpMessage tsyn SB" where
 "aBP_sender_ds__mediumSr_ar sender_port_ds__mediumSr_port_ar = sbe2SB (aBPElem_sender_ds__mediumSr_ar sender_port_ds__mediumSr_port_ar)"
 
 (* Do not use this, use aBPMediumSrElemOut_as or aBPReceiverElemIn_dr instead *)
-fun aBPElem_mediumSr_as__receiver_dr :: "('e×bool) tsyn ⇒ ('e::countable) abpMessage tsyn sbElem" where
+fun aBPElem_mediumSr_as__receiver_dr :: "('e\<times>bool) tsyn \<Rightarrow> ('e::countable) abpMessage tsyn sbElem" where
 "aBPElem_mediumSr_as__receiver_dr (Msg mediumSr_port_as__receiver_port_dr) = aBPElem_raw_mediumSr_as__receiver_dr mediumSr_port_as__receiver_port_dr" |
-"aBPElem_mediumSr_as__receiver_dr null = sbeNull {𝒞 ''DoNotUse_65e4c1937d484f20baf2707bdccbfc49_mediumSr_as__receiver_dr''}"
+"aBPElem_mediumSr_as__receiver_dr null = sbeNull {\<C> ''mediumSr_as__receiver_dr''}"
 
 declare aBPElem_mediumSr_as__receiver_dr.simps[simp del]
 
 (* Do not use this, use aBPMediumSrOut_as or aBPReceiverIn_dr instead *)
-definition aBP_mediumSr_as__receiver_dr :: "('e×bool) tsyn ⇒ ('e::countable) abpMessage tsyn SB" where
+definition aBP_mediumSr_as__receiver_dr :: "('e\<times>bool) tsyn \<Rightarrow> ('e::countable) abpMessage tsyn SB" where
 "aBP_mediumSr_as__receiver_dr mediumSr_port_as__receiver_port_dr = sbe2SB (aBPElem_mediumSr_as__receiver_dr mediumSr_port_as__receiver_port_dr)"
 
 (* Do not use this, use aBPReceiverElemOut_ar_o or aBPMediumRsElemIn_ar instead *)
-fun aBPElem_receiver_ar__mediumRs_ar :: "bool tsyn ⇒ ('e::countable) abpMessage tsyn sbElem" where
+fun aBPElem_receiver_ar__mediumRs_ar :: "bool tsyn \<Rightarrow> ('e::countable) abpMessage tsyn sbElem" where
 "aBPElem_receiver_ar__mediumRs_ar (Msg receiver_port_ar__mediumRs_port_ar) = aBPElem_raw_receiver_ar__mediumRs_ar receiver_port_ar__mediumRs_port_ar" |
-"aBPElem_receiver_ar__mediumRs_ar null = sbeNull {𝒞 ''DoNotUse_65e4c1937d484f20baf2707bdccbfc49_receiver_ar__mediumRs_ar''}"
+"aBPElem_receiver_ar__mediumRs_ar null = sbeNull {\<C> ''receiver_ar__mediumRs_ar''}"
 
 declare aBPElem_receiver_ar__mediumRs_ar.simps[simp del]
 
 (* Do not use this, use aBPReceiverOut_ar_o or aBPMediumRsIn_ar instead *)
-definition aBP_receiver_ar__mediumRs_ar :: "bool tsyn ⇒ ('e::countable) abpMessage tsyn SB" where
+definition aBP_receiver_ar__mediumRs_ar :: "bool tsyn \<Rightarrow> ('e::countable) abpMessage tsyn SB" where
 "aBP_receiver_ar__mediumRs_ar receiver_port_ar__mediumRs_port_ar = sbe2SB (aBPElem_receiver_ar__mediumRs_ar receiver_port_ar__mediumRs_port_ar)"
 
 (* Do not use this, use aBPMediumRsElemOut_as or aBPSenderElemIn_as_i instead *)
-fun aBPElem_mediumRs_as__sender_as :: "bool tsyn ⇒ ('e::countable) abpMessage tsyn sbElem" where
+fun aBPElem_mediumRs_as__sender_as :: "bool tsyn \<Rightarrow> ('e::countable) abpMessage tsyn sbElem" where
 "aBPElem_mediumRs_as__sender_as (Msg mediumRs_port_as__sender_port_as) = aBPElem_raw_mediumRs_as__sender_as mediumRs_port_as__sender_port_as" |
-"aBPElem_mediumRs_as__sender_as null = sbeNull {𝒞 ''DoNotUse_65e4c1937d484f20baf2707bdccbfc49_mediumRs_as__sender_as''}"
+"aBPElem_mediumRs_as__sender_as null = sbeNull {\<C> ''mediumRs_as__sender_as''}"
 
 declare aBPElem_mediumRs_as__sender_as.simps[simp del]
 
 (* Do not use this, use aBPMediumRsOut_as or aBPSenderIn_as_i instead *)
-definition aBP_mediumRs_as__sender_as :: "bool tsyn ⇒ ('e::countable) abpMessage tsyn SB" where
+definition aBP_mediumRs_as__sender_as :: "bool tsyn \<Rightarrow> ('e::countable) abpMessage tsyn SB" where
 "aBP_mediumRs_as__sender_as mediumRs_port_as__sender_port_as = sbe2SB (aBPElem_mediumRs_as__sender_as mediumRs_port_as__sender_port_as)"
 
 (* Create one sbElem for all input channels *)
-definition aBPElemIn_i :: "'e tsyn ⇒ ('e::countable) abpMessage tsyn sbElem" where
+definition aBPElemIn_i :: "'e tsyn \<Rightarrow> ('e::countable) abpMessage tsyn sbElem" where
 "aBPElemIn_i port_i = (aBPElem_i__sender_i port_i)"
 
 (* Create one sbElem for all output channels *)
-definition aBPElemOut_o :: "'e tsyn ⇒ ('e::countable) abpMessage tsyn sbElem" where
+definition aBPElemOut_o :: "'e tsyn \<Rightarrow> ('e::countable) abpMessage tsyn sbElem" where
 "aBPElemOut_o port_o = (aBPElem_receiver_o__o port_o)"
 
 (* Create one SB for all input channels *)
-definition aBPIn_i :: "'e tsyn ⇒ ('e::countable) abpMessage tsyn SB" where
+definition aBPIn_i :: "'e tsyn \<Rightarrow> ('e::countable) abpMessage tsyn SB" where
 "aBPIn_i port_i = (sbe2SB (aBPElemIn_i port_i))"
 
 (* Create one SB for all output channels *)
-definition aBPOut_o :: "'e tsyn ⇒ ('e::countable) abpMessage tsyn SB" where
+definition aBPOut_o :: "'e tsyn \<Rightarrow> ('e::countable) abpMessage tsyn SB" where
 "aBPOut_o port_o = (sbe2SB (aBPElemOut_o port_o))"
 
 
-subsection ‹sender›
+subsection \<open>sender\<close>
 
 (* Create one sbElem for all input channels *)
-definition aBPSenderElemIn_as_i :: "bool tsyn ⇒ 'e tsyn ⇒ ('e::countable) abpMessage tsyn sbElem" where
-"aBPSenderElemIn_as_i port_as port_i = (aBPElem_mediumRs_as__sender_as port_as) ± (aBPElem_i__sender_i port_i)"
+definition aBPSenderElemIn_as_i :: "bool tsyn \<Rightarrow> 'e tsyn \<Rightarrow> ('e::countable) abpMessage tsyn sbElem" where
+"aBPSenderElemIn_as_i port_as port_i = (aBPElem_mediumRs_as__sender_as port_as) \<plusminus> (aBPElem_i__sender_i port_i)"
 
 (* Create one sbElem for all output channels *)
-definition aBPSenderElemOut_ds :: "('e×bool) tsyn ⇒ ('e::countable) abpMessage tsyn sbElem" where
+definition aBPSenderElemOut_ds :: "('e\<times>bool) tsyn \<Rightarrow> ('e::countable) abpMessage tsyn sbElem" where
 "aBPSenderElemOut_ds port_ds = (aBPElem_sender_ds__mediumSr_ar port_ds)"
 
 (* Create one SB for all input channels *)
-definition aBPSenderIn_as_i :: "bool tsyn ⇒ 'e tsyn ⇒ ('e::countable) abpMessage tsyn SB" where
+definition aBPSenderIn_as_i :: "bool tsyn \<Rightarrow> 'e tsyn \<Rightarrow> ('e::countable) abpMessage tsyn SB" where
 "aBPSenderIn_as_i port_as port_i = (sbe2SB (aBPSenderElemIn_as_i port_as port_i))"
 
 (* Create one SB for all output channels *)
-definition aBPSenderOut_ds :: "('e×bool) tsyn ⇒ ('e::countable) abpMessage tsyn SB" where
+definition aBPSenderOut_ds :: "('e\<times>bool) tsyn \<Rightarrow> ('e::countable) abpMessage tsyn SB" where
 "aBPSenderOut_ds port_ds = (sbe2SB (aBPSenderElemOut_ds port_ds))"
 
 
-subsection ‹mediumSr›
+subsection \<open>mediumSr\<close>
 
 (* Create one sbElem for all input channels *)
-definition aBPMediumSrElemIn_ar :: "('e×bool) tsyn ⇒ ('e::countable) abpMessage tsyn sbElem" where
+definition aBPMediumSrElemIn_ar :: "('e\<times>bool) tsyn \<Rightarrow> ('e::countable) abpMessage tsyn sbElem" where
 "aBPMediumSrElemIn_ar port_ar = (aBPElem_sender_ds__mediumSr_ar port_ar)"
 
 (* Create one sbElem for all output channels *)
-definition aBPMediumSrElemOut_as :: "('e×bool) tsyn ⇒ ('e::countable) abpMessage tsyn sbElem" where
+definition aBPMediumSrElemOut_as :: "('e\<times>bool) tsyn \<Rightarrow> ('e::countable) abpMessage tsyn sbElem" where
 "aBPMediumSrElemOut_as port_as = (aBPElem_mediumSr_as__receiver_dr port_as)"
 
 (* Create one SB for all input channels *)
-definition aBPMediumSrIn_ar :: "('e×bool) tsyn ⇒ ('e::countable) abpMessage tsyn SB" where
+definition aBPMediumSrIn_ar :: "('e\<times>bool) tsyn \<Rightarrow> ('e::countable) abpMessage tsyn SB" where
 "aBPMediumSrIn_ar port_ar = (sbe2SB (aBPMediumSrElemIn_ar port_ar))"
 
 (* Create one SB for all output channels *)
-definition aBPMediumSrOut_as :: "('e×bool) tsyn ⇒ ('e::countable) abpMessage tsyn SB" where
+definition aBPMediumSrOut_as :: "('e\<times>bool) tsyn \<Rightarrow> ('e::countable) abpMessage tsyn SB" where
 "aBPMediumSrOut_as port_as = (sbe2SB (aBPMediumSrElemOut_as port_as))"
 
 
-subsection ‹receiver›
+subsection \<open>receiver\<close>
 
 (* Create one sbElem for all input channels *)
-definition aBPReceiverElemIn_dr :: "('e×bool) tsyn ⇒ ('e::countable) abpMessage tsyn sbElem" where
+definition aBPReceiverElemIn_dr :: "('e\<times>bool) tsyn \<Rightarrow> ('e::countable) abpMessage tsyn sbElem" where
 "aBPReceiverElemIn_dr port_dr = (aBPElem_mediumSr_as__receiver_dr port_dr)"
 
 (* Create one sbElem for all output channels *)
-definition aBPReceiverElemOut_ar_o :: "bool tsyn ⇒ 'e tsyn ⇒ ('e::countable) abpMessage tsyn sbElem" where
-"aBPReceiverElemOut_ar_o port_ar port_o = (aBPElem_receiver_ar__mediumRs_ar port_ar) ± (aBPElem_receiver_o__o port_o)"
+definition aBPReceiverElemOut_ar_o :: "bool tsyn \<Rightarrow> 'e tsyn \<Rightarrow> ('e::countable) abpMessage tsyn sbElem" where
+"aBPReceiverElemOut_ar_o port_ar port_o = (aBPElem_receiver_ar__mediumRs_ar port_ar) \<plusminus> (aBPElem_receiver_o__o port_o)"
 
 (* Create one SB for all input channels *)
-definition aBPReceiverIn_dr :: "('e×bool) tsyn ⇒ ('e::countable) abpMessage tsyn SB" where
+definition aBPReceiverIn_dr :: "('e\<times>bool) tsyn \<Rightarrow> ('e::countable) abpMessage tsyn SB" where
 "aBPReceiverIn_dr port_dr = (sbe2SB (aBPReceiverElemIn_dr port_dr))"
 
 (* Create one SB for all output channels *)
-definition aBPReceiverOut_ar_o :: "bool tsyn ⇒ 'e tsyn ⇒ ('e::countable) abpMessage tsyn SB" where
+definition aBPReceiverOut_ar_o :: "bool tsyn \<Rightarrow> 'e tsyn \<Rightarrow> ('e::countable) abpMessage tsyn SB" where
 "aBPReceiverOut_ar_o port_ar port_o = (sbe2SB (aBPReceiverElemOut_ar_o port_ar port_o))"
 
 
-subsection ‹mediumRs›
+subsection \<open>mediumRs\<close>
 
 (* Create one sbElem for all input channels *)
-definition aBPMediumRsElemIn_ar :: "bool tsyn ⇒ ('e::countable) abpMessage tsyn sbElem" where
+definition aBPMediumRsElemIn_ar :: "bool tsyn \<Rightarrow> ('e::countable) abpMessage tsyn sbElem" where
 "aBPMediumRsElemIn_ar port_ar = (aBPElem_receiver_ar__mediumRs_ar port_ar)"
 
 (* Create one sbElem for all output channels *)
-definition aBPMediumRsElemOut_as :: "bool tsyn ⇒ ('e::countable) abpMessage tsyn sbElem" where
+definition aBPMediumRsElemOut_as :: "bool tsyn \<Rightarrow> ('e::countable) abpMessage tsyn sbElem" where
 "aBPMediumRsElemOut_as port_as = (aBPElem_mediumRs_as__sender_as port_as)"
 
 (* Create one SB for all input channels *)
-definition aBPMediumRsIn_ar :: "bool tsyn ⇒ ('e::countable) abpMessage tsyn SB" where
+definition aBPMediumRsIn_ar :: "bool tsyn \<Rightarrow> ('e::countable) abpMessage tsyn SB" where
 "aBPMediumRsIn_ar port_ar = (sbe2SB (aBPMediumRsElemIn_ar port_ar))"
 
 (* Create one SB for all output channels *)
-definition aBPMediumRsOut_as :: "bool tsyn ⇒ ('e::countable) abpMessage tsyn SB" where
+definition aBPMediumRsOut_as :: "bool tsyn \<Rightarrow> ('e::countable) abpMessage tsyn SB" where
 "aBPMediumRsOut_as port_as = (sbe2SB (aBPMediumRsElemOut_as port_as))"
 
 
-section ‹Helpers to create a bundle from a tsyn list of elements›
+section \<open>Helpers to create a bundle from a tsyn list of elements\<close>
 
 (* Do not use this, use aBPReceiverOut_list_ar_o or aBPOut_list_o instead *)
-fun aBP_list_receiver_o__o :: "('e tsyn) list ⇒ ('e::countable) abpMessage tsyn SB" where
-"aBP_list_receiver_o__o (x#xs) = ubConcEq (aBP_receiver_o__o x)⋅(aBP_list_receiver_o__o xs)" |
-"aBP_list_receiver_o__o []     = ubLeast {𝒞 ''DoNotUse_65e4c1937d484f20baf2707bdccbfc49_receiver_o__o''}"
+fun aBP_list_receiver_o__o :: "('e tsyn) list \<Rightarrow> ('e::countable) abpMessage tsyn SB" where
+"aBP_list_receiver_o__o (x#xs) = ubConcEq (aBP_receiver_o__o x)\<cdot>(aBP_list_receiver_o__o xs)" |
+"aBP_list_receiver_o__o []     = ubLeast {\<C> ''receiver_o__o''}"
 
 declare aBP_list_receiver_o__o.simps[simp del]
 
 (* Do not use this, use aBPIn_list_i or aBPSenderIn_list_as_i instead *)
-fun aBP_list_i__sender_i :: "('e tsyn) list ⇒ ('e::countable) abpMessage tsyn SB" where
-"aBP_list_i__sender_i (x#xs) = ubConcEq (aBP_i__sender_i x)⋅(aBP_list_i__sender_i xs)" |
-"aBP_list_i__sender_i []     = ubLeast {𝒞 ''DoNotUse_65e4c1937d484f20baf2707bdccbfc49_i__sender_i''}"
+fun aBP_list_i__sender_i :: "('e tsyn) list \<Rightarrow> ('e::countable) abpMessage tsyn SB" where
+"aBP_list_i__sender_i (x#xs) = ubConcEq (aBP_i__sender_i x)\<cdot>(aBP_list_i__sender_i xs)" |
+"aBP_list_i__sender_i []     = ubLeast {\<C> ''i__sender_i''}"
 
 declare aBP_list_i__sender_i.simps[simp del]
 
 (* Do not use this, use aBPSenderOut_list_ds or aBPMediumSrIn_list_ar instead *)
-fun aBP_list_sender_ds__mediumSr_ar :: "(('e×bool) tsyn) list ⇒ ('e::countable) abpMessage tsyn SB" where
-"aBP_list_sender_ds__mediumSr_ar (x#xs) = ubConcEq (aBP_sender_ds__mediumSr_ar x)⋅(aBP_list_sender_ds__mediumSr_ar xs)" |
-"aBP_list_sender_ds__mediumSr_ar []     = ubLeast {𝒞 ''DoNotUse_65e4c1937d484f20baf2707bdccbfc49_sender_ds__mediumSr_ar''}"
+fun aBP_list_sender_ds__mediumSr_ar :: "(('e\<times>bool) tsyn) list \<Rightarrow> ('e::countable) abpMessage tsyn SB" where
+"aBP_list_sender_ds__mediumSr_ar (x#xs) = ubConcEq (aBP_sender_ds__mediumSr_ar x)\<cdot>(aBP_list_sender_ds__mediumSr_ar xs)" |
+"aBP_list_sender_ds__mediumSr_ar []     = ubLeast {\<C> ''sender_ds__mediumSr_ar''}"
 
 declare aBP_list_sender_ds__mediumSr_ar.simps[simp del]
 
 (* Do not use this, use aBPMediumSrOut_list_as or aBPReceiverIn_list_dr instead *)
-fun aBP_list_mediumSr_as__receiver_dr :: "(('e×bool) tsyn) list ⇒ ('e::countable) abpMessage tsyn SB" where
-"aBP_list_mediumSr_as__receiver_dr (x#xs) = ubConcEq (aBP_mediumSr_as__receiver_dr x)⋅(aBP_list_mediumSr_as__receiver_dr xs)" |
-"aBP_list_mediumSr_as__receiver_dr []     = ubLeast {𝒞 ''DoNotUse_65e4c1937d484f20baf2707bdccbfc49_mediumSr_as__receiver_dr''}"
+fun aBP_list_mediumSr_as__receiver_dr :: "(('e\<times>bool) tsyn) list \<Rightarrow> ('e::countable) abpMessage tsyn SB" where
+"aBP_list_mediumSr_as__receiver_dr (x#xs) = ubConcEq (aBP_mediumSr_as__receiver_dr x)\<cdot>(aBP_list_mediumSr_as__receiver_dr xs)" |
+"aBP_list_mediumSr_as__receiver_dr []     = ubLeast {\<C> ''mediumSr_as__receiver_dr''}"
 
 declare aBP_list_mediumSr_as__receiver_dr.simps[simp del]
 
 (* Do not use this, use aBPReceiverOut_list_ar_o or aBPMediumRsIn_list_ar instead *)
-fun aBP_list_receiver_ar__mediumRs_ar :: "(bool tsyn) list ⇒ ('e::countable) abpMessage tsyn SB" where
-"aBP_list_receiver_ar__mediumRs_ar (x#xs) = ubConcEq (aBP_receiver_ar__mediumRs_ar x)⋅(aBP_list_receiver_ar__mediumRs_ar xs)" |
-"aBP_list_receiver_ar__mediumRs_ar []     = ubLeast {𝒞 ''DoNotUse_65e4c1937d484f20baf2707bdccbfc49_receiver_ar__mediumRs_ar''}"
+fun aBP_list_receiver_ar__mediumRs_ar :: "(bool tsyn) list \<Rightarrow> ('e::countable) abpMessage tsyn SB" where
+"aBP_list_receiver_ar__mediumRs_ar (x#xs) = ubConcEq (aBP_receiver_ar__mediumRs_ar x)\<cdot>(aBP_list_receiver_ar__mediumRs_ar xs)" |
+"aBP_list_receiver_ar__mediumRs_ar []     = ubLeast {\<C> ''receiver_ar__mediumRs_ar''}"
 
 declare aBP_list_receiver_ar__mediumRs_ar.simps[simp del]
 
 (* Do not use this, use aBPMediumRsOut_list_as or aBPSenderIn_list_as_i instead *)
-fun aBP_list_mediumRs_as__sender_as :: "(bool tsyn) list ⇒ ('e::countable) abpMessage tsyn SB" where
-"aBP_list_mediumRs_as__sender_as (x#xs) = ubConcEq (aBP_mediumRs_as__sender_as x)⋅(aBP_list_mediumRs_as__sender_as xs)" |
-"aBP_list_mediumRs_as__sender_as []     = ubLeast {𝒞 ''DoNotUse_65e4c1937d484f20baf2707bdccbfc49_mediumRs_as__sender_as''}"
+fun aBP_list_mediumRs_as__sender_as :: "(bool tsyn) list \<Rightarrow> ('e::countable) abpMessage tsyn SB" where
+"aBP_list_mediumRs_as__sender_as (x#xs) = ubConcEq (aBP_mediumRs_as__sender_as x)\<cdot>(aBP_list_mediumRs_as__sender_as xs)" |
+"aBP_list_mediumRs_as__sender_as []     = ubLeast {\<C> ''mediumRs_as__sender_as''}"
 
 declare aBP_list_mediumRs_as__sender_as.simps[simp del]
 
 (* Create one SB for all input channels *)
-fun aBPIn_list_i :: "('e tsyn) list ⇒ ('e::countable) abpMessage tsyn SB" where
-"aBPIn_list_i ((port_i)#xs) = ubConcEq (aBPIn_i port_i)⋅(aBPIn_list_i xs)" |
+fun aBPIn_list_i :: "('e tsyn) list \<Rightarrow> ('e::countable) abpMessage tsyn SB" where
+"aBPIn_list_i ((port_i)#xs) = ubConcEq (aBPIn_i port_i)\<cdot>(aBPIn_list_i xs)" |
 "aBPIn_list_i [] = ubLeast aBPDom"
 
 (* Create one SB for all output channels *)
-fun aBPOut_list_o :: "('e tsyn) list ⇒ ('e::countable) abpMessage tsyn SB" where
-"aBPOut_list_o ((port_o)#xs) = ubConcEq (aBPOut_o port_o)⋅(aBPOut_list_o xs)" |
+fun aBPOut_list_o :: "('e tsyn) list \<Rightarrow> ('e::countable) abpMessage tsyn SB" where
+"aBPOut_list_o ((port_o)#xs) = ubConcEq (aBPOut_o port_o)\<cdot>(aBPOut_list_o xs)" |
 "aBPOut_list_o [] = ubLeast aBPRan"
 
 
-subsection ‹sender›
+subsection \<open>sender\<close>
 
 (* Create one SB for all input channels *)
-fun aBPSenderIn_list_as_i :: "(bool tsyn×'e tsyn) list ⇒ ('e::countable) abpMessage tsyn SB" where
-"aBPSenderIn_list_as_i ((port_as,port_i)#xs) = ubConcEq (aBPSenderIn_as_i port_as port_i)⋅(aBPSenderIn_list_as_i xs)" |
+fun aBPSenderIn_list_as_i :: "(bool tsyn\<times>'e tsyn) list \<Rightarrow> ('e::countable) abpMessage tsyn SB" where
+"aBPSenderIn_list_as_i ((port_as,port_i)#xs) = ubConcEq (aBPSenderIn_as_i port_as port_i)\<cdot>(aBPSenderIn_list_as_i xs)" |
 "aBPSenderIn_list_as_i [] = ubLeast aBPSenderDom"
 
 (* Create one SB for all output channels *)
-fun aBPSenderOut_list_ds :: "(('e×bool) tsyn) list ⇒ ('e::countable) abpMessage tsyn SB" where
-"aBPSenderOut_list_ds ((port_ds)#xs) = ubConcEq (aBPSenderOut_ds port_ds)⋅(aBPSenderOut_list_ds xs)" |
+fun aBPSenderOut_list_ds :: "(('e\<times>bool) tsyn) list \<Rightarrow> ('e::countable) abpMessage tsyn SB" where
+"aBPSenderOut_list_ds ((port_ds)#xs) = ubConcEq (aBPSenderOut_ds port_ds)\<cdot>(aBPSenderOut_list_ds xs)" |
 "aBPSenderOut_list_ds [] = ubLeast aBPSenderRan"
 
 
-subsection ‹mediumSr›
+subsection \<open>mediumSr\<close>
 
 (* Create one SB for all input channels *)
-fun aBPMediumSrIn_list_ar :: "(('e×bool) tsyn) list ⇒ ('e::countable) abpMessage tsyn SB" where
-"aBPMediumSrIn_list_ar ((port_ar)#xs) = ubConcEq (aBPMediumSrIn_ar port_ar)⋅(aBPMediumSrIn_list_ar xs)" |
+fun aBPMediumSrIn_list_ar :: "(('e\<times>bool) tsyn) list \<Rightarrow> ('e::countable) abpMessage tsyn SB" where
+"aBPMediumSrIn_list_ar ((port_ar)#xs) = ubConcEq (aBPMediumSrIn_ar port_ar)\<cdot>(aBPMediumSrIn_list_ar xs)" |
 "aBPMediumSrIn_list_ar [] = ubLeast aBPMediumSrDom"
 
 (* Create one SB for all output channels *)
-fun aBPMediumSrOut_list_as :: "(('e×bool) tsyn) list ⇒ ('e::countable) abpMessage tsyn SB" where
-"aBPMediumSrOut_list_as ((port_as)#xs) = ubConcEq (aBPMediumSrOut_as port_as)⋅(aBPMediumSrOut_list_as xs)" |
+fun aBPMediumSrOut_list_as :: "(('e\<times>bool) tsyn) list \<Rightarrow> ('e::countable) abpMessage tsyn SB" where
+"aBPMediumSrOut_list_as ((port_as)#xs) = ubConcEq (aBPMediumSrOut_as port_as)\<cdot>(aBPMediumSrOut_list_as xs)" |
 "aBPMediumSrOut_list_as [] = ubLeast aBPMediumSrRan"
 
 
-subsection ‹receiver›
+subsection \<open>receiver\<close>
 
 (* Create one SB for all input channels *)
-fun aBPReceiverIn_list_dr :: "(('e×bool) tsyn) list ⇒ ('e::countable) abpMessage tsyn SB" where
-"aBPReceiverIn_list_dr ((port_dr)#xs) = ubConcEq (aBPReceiverIn_dr port_dr)⋅(aBPReceiverIn_list_dr xs)" |
+fun aBPReceiverIn_list_dr :: "(('e\<times>bool) tsyn) list \<Rightarrow> ('e::countable) abpMessage tsyn SB" where
+"aBPReceiverIn_list_dr ((port_dr)#xs) = ubConcEq (aBPReceiverIn_dr port_dr)\<cdot>(aBPReceiverIn_list_dr xs)" |
 "aBPReceiverIn_list_dr [] = ubLeast aBPReceiverDom"
 
 (* Create one SB for all output channels *)
-fun aBPReceiverOut_list_ar_o :: "(bool tsyn×'e tsyn) list ⇒ ('e::countable) abpMessage tsyn SB" where
-"aBPReceiverOut_list_ar_o ((port_ar,port_o)#xs) = ubConcEq (aBPReceiverOut_ar_o port_ar port_o)⋅(aBPReceiverOut_list_ar_o xs)" |
+fun aBPReceiverOut_list_ar_o :: "(bool tsyn\<times>'e tsyn) list \<Rightarrow> ('e::countable) abpMessage tsyn SB" where
+"aBPReceiverOut_list_ar_o ((port_ar,port_o)#xs) = ubConcEq (aBPReceiverOut_ar_o port_ar port_o)\<cdot>(aBPReceiverOut_list_ar_o xs)" |
 "aBPReceiverOut_list_ar_o [] = ubLeast aBPReceiverRan"
 
 
-subsection ‹mediumRs›
+subsection \<open>mediumRs\<close>
 
 (* Create one SB for all input channels *)
-fun aBPMediumRsIn_list_ar :: "(bool tsyn) list ⇒ ('e::countable) abpMessage tsyn SB" where
-"aBPMediumRsIn_list_ar ((port_ar)#xs) = ubConcEq (aBPMediumRsIn_ar port_ar)⋅(aBPMediumRsIn_list_ar xs)" |
+fun aBPMediumRsIn_list_ar :: "(bool tsyn) list \<Rightarrow> ('e::countable) abpMessage tsyn SB" where
+"aBPMediumRsIn_list_ar ((port_ar)#xs) = ubConcEq (aBPMediumRsIn_ar port_ar)\<cdot>(aBPMediumRsIn_list_ar xs)" |
 "aBPMediumRsIn_list_ar [] = ubLeast aBPMediumRsDom"
 
 (* Create one SB for all output channels *)
-fun aBPMediumRsOut_list_as :: "(bool tsyn) list ⇒ ('e::countable) abpMessage tsyn SB" where
-"aBPMediumRsOut_list_as ((port_as)#xs) = ubConcEq (aBPMediumRsOut_as port_as)⋅(aBPMediumRsOut_list_as xs)" |
+fun aBPMediumRsOut_list_as :: "(bool tsyn) list \<Rightarrow> ('e::countable) abpMessage tsyn SB" where
+"aBPMediumRsOut_list_as ((port_as)#xs) = ubConcEq (aBPMediumRsOut_as port_as)\<cdot>(aBPMediumRsOut_list_as xs)" |
 "aBPMediumRsOut_list_as [] = ubLeast aBPMediumRsRan"
 
 
-section ‹Helpers to create a bundle from a tsyn stream of elements›
+section \<open>Helpers to create a bundle from a tsyn stream of elements\<close>
 
-lift_definition DoNotUse_65e4c1937d484f20baf2707bdccbfc49_aBP_stream_receiver_o__o_h :: "'e tsyn stream ⇒ ('e::countable) abpMessage tsyn SB" is
-"λ s. [(𝒞 ''DoNotUse_65e4c1937d484f20baf2707bdccbfc49_receiver_o__o'') ↦ (tsynMap (DoNotUse_65e4c1937d484f20baf2707bdccbfc49_ABPE)⋅s)]"
+lift_definition aBP_stream_receiver_o__o_h :: "'e tsyn stream \<Rightarrow> ('e::countable) abpMessage tsyn SB" is
+"\<lambda> s. [(\<C> ''receiver_o__o'') \<mapsto> (tsynMap (ABPE)\<cdot>s)]"
   unfolding ubWell_def usclOkay_stream_def ctype_tsyn_def
   by auto
 
 (* Do not use this, use aBPReceiverOut_stream_ar_o or aBPOut_stream_o instead *)
-lift_definition aBP_stream_receiver_o__o :: "('e) tsyn stream → ('e::countable) abpMessage tsyn SB" is
-"DoNotUse_65e4c1937d484f20baf2707bdccbfc49_aBP_stream_receiver_o__o_h"
-  apply(auto simp add: cfun_def DoNotUse_65e4c1937d484f20baf2707bdccbfc49_aBP_stream_receiver_o__o_h_def map_fun_def comp_def)
+lift_definition aBP_stream_receiver_o__o :: "('e) tsyn stream \<rightarrow> ('e::countable) abpMessage tsyn SB" is
+"aBP_stream_receiver_o__o_h"
+  apply(auto simp add: cfun_def aBP_stream_receiver_o__o_h_def map_fun_def comp_def)
   apply(rule cont_Abs_UB)
   apply(simp add: option_one_cont)
-  by (metis DoNotUse_65e4c1937d484f20baf2707bdccbfc49_aBP_stream_receiver_o__o_h.rep_eq ubrep_well)
+  by (metis aBP_stream_receiver_o__o_h.rep_eq ubrep_well)
 
-lift_definition DoNotUse_65e4c1937d484f20baf2707bdccbfc49_aBP_stream_i__sender_i_h :: "'e tsyn stream ⇒ ('e::countable) abpMessage tsyn SB" is
-"λ s. [(𝒞 ''DoNotUse_65e4c1937d484f20baf2707bdccbfc49_i__sender_i'') ↦ (tsynMap (DoNotUse_65e4c1937d484f20baf2707bdccbfc49_ABPE)⋅s)]"
+lift_definition aBP_stream_i__sender_i_h :: "'e tsyn stream \<Rightarrow> ('e::countable) abpMessage tsyn SB" is
+"\<lambda> s. [(\<C> ''i__sender_i'') \<mapsto> (tsynMap (ABPE)\<cdot>s)]"
   unfolding ubWell_def usclOkay_stream_def ctype_tsyn_def
   by auto
 
 (* Do not use this, use aBPIn_stream_i or aBPSenderIn_stream_as_i instead *)
-lift_definition aBP_stream_i__sender_i :: "('e) tsyn stream → ('e::countable) abpMessage tsyn SB" is
-"DoNotUse_65e4c1937d484f20baf2707bdccbfc49_aBP_stream_i__sender_i_h"
-  apply(auto simp add: cfun_def DoNotUse_65e4c1937d484f20baf2707bdccbfc49_aBP_stream_i__sender_i_h_def map_fun_def comp_def)
+lift_definition aBP_stream_i__sender_i :: "('e) tsyn stream \<rightarrow> ('e::countable) abpMessage tsyn SB" is
+"aBP_stream_i__sender_i_h"
+  apply(auto simp add: cfun_def aBP_stream_i__sender_i_h_def map_fun_def comp_def)
   apply(rule cont_Abs_UB)
   apply(simp add: option_one_cont)
-  by (metis DoNotUse_65e4c1937d484f20baf2707bdccbfc49_aBP_stream_i__sender_i_h.rep_eq ubrep_well)
+  by (metis aBP_stream_i__sender_i_h.rep_eq ubrep_well)
 
-lift_definition DoNotUse_65e4c1937d484f20baf2707bdccbfc49_aBP_stream_sender_ds__mediumSr_ar_h :: "('e×bool) tsyn stream ⇒ ('e::countable) abpMessage tsyn SB" is
-"λ s. [(𝒞 ''DoNotUse_65e4c1937d484f20baf2707bdccbfc49_sender_ds__mediumSr_ar'') ↦ (tsynMap (DoNotUse_65e4c1937d484f20baf2707bdccbfc49_ABPPair_E_Bool)⋅s)]"
+lift_definition aBP_stream_sender_ds__mediumSr_ar_h :: "('e\<times>bool) tsyn stream \<Rightarrow> ('e::countable) abpMessage tsyn SB" is
+"\<lambda> s. [(\<C> ''sender_ds__mediumSr_ar'') \<mapsto> (tsynMap (ABPPair_E_Bool)\<cdot>s)]"
   unfolding ubWell_def usclOkay_stream_def ctype_tsyn_def
   by auto
 
 (* Do not use this, use aBPSenderOut_stream_ds or aBPMediumSrIn_stream_ar instead *)
-lift_definition aBP_stream_sender_ds__mediumSr_ar :: "(('e×bool)) tsyn stream → ('e::countable) abpMessage tsyn SB" is
-"DoNotUse_65e4c1937d484f20baf2707bdccbfc49_aBP_stream_sender_ds__mediumSr_ar_h"
-  apply(auto simp add: cfun_def DoNotUse_65e4c1937d484f20baf2707bdccbfc49_aBP_stream_sender_ds__mediumSr_ar_h_def map_fun_def comp_def)
+lift_definition aBP_stream_sender_ds__mediumSr_ar :: "(('e\<times>bool)) tsyn stream \<rightarrow> ('e::countable) abpMessage tsyn SB" is
+"aBP_stream_sender_ds__mediumSr_ar_h"
+  apply(auto simp add: cfun_def aBP_stream_sender_ds__mediumSr_ar_h_def map_fun_def comp_def)
   apply(rule cont_Abs_UB)
   apply(simp add: option_one_cont)
-  by (metis DoNotUse_65e4c1937d484f20baf2707bdccbfc49_aBP_stream_sender_ds__mediumSr_ar_h.rep_eq ubrep_well)
+  by (metis aBP_stream_sender_ds__mediumSr_ar_h.rep_eq ubrep_well)
 
-lift_definition DoNotUse_65e4c1937d484f20baf2707bdccbfc49_aBP_stream_mediumSr_as__receiver_dr_h :: "('e×bool) tsyn stream ⇒ ('e::countable) abpMessage tsyn SB" is
-"λ s. [(𝒞 ''DoNotUse_65e4c1937d484f20baf2707bdccbfc49_mediumSr_as__receiver_dr'') ↦ (tsynMap (DoNotUse_65e4c1937d484f20baf2707bdccbfc49_ABPPair_E_Bool)⋅s)]"
+lift_definition aBP_stream_mediumSr_as__receiver_dr_h :: "('e\<times>bool) tsyn stream \<Rightarrow> ('e::countable) abpMessage tsyn SB" is
+"\<lambda> s. [(\<C> ''mediumSr_as__receiver_dr'') \<mapsto> (tsynMap (ABPPair_E_Bool)\<cdot>s)]"
   unfolding ubWell_def usclOkay_stream_def ctype_tsyn_def
   by auto
 
 (* Do not use this, use aBPMediumSrOut_stream_as or aBPReceiverIn_stream_dr instead *)
-lift_definition aBP_stream_mediumSr_as__receiver_dr :: "(('e×bool)) tsyn stream → ('e::countable) abpMessage tsyn SB" is
-"DoNotUse_65e4c1937d484f20baf2707bdccbfc49_aBP_stream_mediumSr_as__receiver_dr_h"
-  apply(auto simp add: cfun_def DoNotUse_65e4c1937d484f20baf2707bdccbfc49_aBP_stream_mediumSr_as__receiver_dr_h_def map_fun_def comp_def)
+lift_definition aBP_stream_mediumSr_as__receiver_dr :: "(('e\<times>bool)) tsyn stream \<rightarrow> ('e::countable) abpMessage tsyn SB" is
+"aBP_stream_mediumSr_as__receiver_dr_h"
+  apply(auto simp add: cfun_def aBP_stream_mediumSr_as__receiver_dr_h_def map_fun_def comp_def)
   apply(rule cont_Abs_UB)
   apply(simp add: option_one_cont)
-  by (metis DoNotUse_65e4c1937d484f20baf2707bdccbfc49_aBP_stream_mediumSr_as__receiver_dr_h.rep_eq ubrep_well)
+  by (metis aBP_stream_mediumSr_as__receiver_dr_h.rep_eq ubrep_well)
 
-lift_definition DoNotUse_65e4c1937d484f20baf2707bdccbfc49_aBP_stream_receiver_ar__mediumRs_ar_h :: "bool tsyn stream ⇒ ('e::countable) abpMessage tsyn SB" is
-"λ s. [(𝒞 ''DoNotUse_65e4c1937d484f20baf2707bdccbfc49_receiver_ar__mediumRs_ar'') ↦ (tsynMap (DoNotUse_65e4c1937d484f20baf2707bdccbfc49_ABPBool)⋅s)]"
+lift_definition aBP_stream_receiver_ar__mediumRs_ar_h :: "bool tsyn stream \<Rightarrow> ('e::countable) abpMessage tsyn SB" is
+"\<lambda> s. [(\<C> ''receiver_ar__mediumRs_ar'') \<mapsto> (tsynMap (ABPBool)\<cdot>s)]"
   unfolding ubWell_def usclOkay_stream_def ctype_tsyn_def
   by auto
 
 (* Do not use this, use aBPReceiverOut_stream_ar_o or aBPMediumRsIn_stream_ar instead *)
-lift_definition aBP_stream_receiver_ar__mediumRs_ar :: "(bool) tsyn stream → ('e::countable) abpMessage tsyn SB" is
-"DoNotUse_65e4c1937d484f20baf2707bdccbfc49_aBP_stream_receiver_ar__mediumRs_ar_h"
-  apply(auto simp add: cfun_def DoNotUse_65e4c1937d484f20baf2707bdccbfc49_aBP_stream_receiver_ar__mediumRs_ar_h_def map_fun_def comp_def)
+lift_definition aBP_stream_receiver_ar__mediumRs_ar :: "(bool) tsyn stream \<rightarrow> ('e::countable) abpMessage tsyn SB" is
+"aBP_stream_receiver_ar__mediumRs_ar_h"
+  apply(auto simp add: cfun_def aBP_stream_receiver_ar__mediumRs_ar_h_def map_fun_def comp_def)
   apply(rule cont_Abs_UB)
   apply(simp add: option_one_cont)
-  by (metis DoNotUse_65e4c1937d484f20baf2707bdccbfc49_aBP_stream_receiver_ar__mediumRs_ar_h.rep_eq ubrep_well)
+  by (metis aBP_stream_receiver_ar__mediumRs_ar_h.rep_eq ubrep_well)
 
-lift_definition DoNotUse_65e4c1937d484f20baf2707bdccbfc49_aBP_stream_mediumRs_as__sender_as_h :: "bool tsyn stream ⇒ ('e::countable) abpMessage tsyn SB" is
-"λ s. [(𝒞 ''DoNotUse_65e4c1937d484f20baf2707bdccbfc49_mediumRs_as__sender_as'') ↦ (tsynMap (DoNotUse_65e4c1937d484f20baf2707bdccbfc49_ABPBool)⋅s)]"
+lift_definition aBP_stream_mediumRs_as__sender_as_h :: "bool tsyn stream \<Rightarrow> ('e::countable) abpMessage tsyn SB" is
+"\<lambda> s. [(\<C> ''mediumRs_as__sender_as'') \<mapsto> (tsynMap (ABPBool)\<cdot>s)]"
   unfolding ubWell_def usclOkay_stream_def ctype_tsyn_def
   by auto
 
 (* Do not use this, use aBPMediumRsOut_stream_as or aBPSenderIn_stream_as_i instead *)
-lift_definition aBP_stream_mediumRs_as__sender_as :: "(bool) tsyn stream → ('e::countable) abpMessage tsyn SB" is
-"DoNotUse_65e4c1937d484f20baf2707bdccbfc49_aBP_stream_mediumRs_as__sender_as_h"
-  apply(auto simp add: cfun_def DoNotUse_65e4c1937d484f20baf2707bdccbfc49_aBP_stream_mediumRs_as__sender_as_h_def map_fun_def comp_def)
+lift_definition aBP_stream_mediumRs_as__sender_as :: "(bool) tsyn stream \<rightarrow> ('e::countable) abpMessage tsyn SB" is
+"aBP_stream_mediumRs_as__sender_as_h"
+  apply(auto simp add: cfun_def aBP_stream_mediumRs_as__sender_as_h_def map_fun_def comp_def)
   apply(rule cont_Abs_UB)
   apply(simp add: option_one_cont)
-  by (metis DoNotUse_65e4c1937d484f20baf2707bdccbfc49_aBP_stream_mediumRs_as__sender_as_h.rep_eq ubrep_well)
+  by (metis aBP_stream_mediumRs_as__sender_as_h.rep_eq ubrep_well)
 
 (* Create one SB for all input channels *)
-definition aBPIn_stream_i :: "'e tsyn stream → ('e::countable) abpMessage tsyn SB" where
-"aBPIn_stream_i = (Λ  port_i. (aBP_stream_i__sender_i⋅port_i))"
+definition aBPIn_stream_i :: "'e tsyn stream \<rightarrow> ('e::countable) abpMessage tsyn SB" where
+"aBPIn_stream_i = (\<Lambda>  port_i. (aBP_stream_i__sender_i\<cdot>port_i))"
 
 (* Create one SB for all output channels *)
-definition aBPOut_stream_o :: "'e tsyn stream → ('e::countable) abpMessage tsyn SB" where
-"aBPOut_stream_o = (Λ  port_o. (aBP_stream_receiver_o__o⋅port_o))"
+definition aBPOut_stream_o :: "'e tsyn stream \<rightarrow> ('e::countable) abpMessage tsyn SB" where
+"aBPOut_stream_o = (\<Lambda>  port_o. (aBP_stream_receiver_o__o\<cdot>port_o))"
 
 
-subsection ‹sender›
+subsection \<open>sender\<close>
 
 (* Create one SB for all input channels *)
-definition aBPSenderIn_stream_as_i :: "bool tsyn stream → 'e tsyn stream → ('e::countable) abpMessage tsyn SB" where
-"aBPSenderIn_stream_as_i = (Λ  port_as port_i. (aBP_stream_mediumRs_as__sender_as⋅port_as) ⊎ (aBP_stream_i__sender_i⋅port_i))"
+definition aBPSenderIn_stream_as_i :: "bool tsyn stream \<rightarrow> 'e tsyn stream \<rightarrow> ('e::countable) abpMessage tsyn SB" where
+"aBPSenderIn_stream_as_i = (\<Lambda>  port_as port_i. (aBP_stream_mediumRs_as__sender_as\<cdot>port_as) \<uplus> (aBP_stream_i__sender_i\<cdot>port_i))"
 
 (* Create one SB for all output channels *)
-definition aBPSenderOut_stream_ds :: "('e×bool) tsyn stream → ('e::countable) abpMessage tsyn SB" where
-"aBPSenderOut_stream_ds = (Λ  port_ds. (aBP_stream_sender_ds__mediumSr_ar⋅port_ds))"
+definition aBPSenderOut_stream_ds :: "('e\<times>bool) tsyn stream \<rightarrow> ('e::countable) abpMessage tsyn SB" where
+"aBPSenderOut_stream_ds = (\<Lambda>  port_ds. (aBP_stream_sender_ds__mediumSr_ar\<cdot>port_ds))"
 
 
-subsection ‹mediumSr›
+subsection \<open>mediumSr\<close>
 
 (* Create one SB for all input channels *)
-definition aBPMediumSrIn_stream_ar :: "('e×bool) tsyn stream → ('e::countable) abpMessage tsyn SB" where
-"aBPMediumSrIn_stream_ar = (Λ  port_ar. (aBP_stream_sender_ds__mediumSr_ar⋅port_ar))"
+definition aBPMediumSrIn_stream_ar :: "('e\<times>bool) tsyn stream \<rightarrow> ('e::countable) abpMessage tsyn SB" where
+"aBPMediumSrIn_stream_ar = (\<Lambda>  port_ar. (aBP_stream_sender_ds__mediumSr_ar\<cdot>port_ar))"
 
 (* Create one SB for all output channels *)
-definition aBPMediumSrOut_stream_as :: "('e×bool) tsyn stream → ('e::countable) abpMessage tsyn SB" where
-"aBPMediumSrOut_stream_as = (Λ  port_as. (aBP_stream_mediumSr_as__receiver_dr⋅port_as))"
+definition aBPMediumSrOut_stream_as :: "('e\<times>bool) tsyn stream \<rightarrow> ('e::countable) abpMessage tsyn SB" where
+"aBPMediumSrOut_stream_as = (\<Lambda>  port_as. (aBP_stream_mediumSr_as__receiver_dr\<cdot>port_as))"
 
 
-subsection ‹receiver›
+subsection \<open>receiver\<close>
 
 (* Create one SB for all input channels *)
-definition aBPReceiverIn_stream_dr :: "('e×bool) tsyn stream → ('e::countable) abpMessage tsyn SB" where
-"aBPReceiverIn_stream_dr = (Λ  port_dr. (aBP_stream_mediumSr_as__receiver_dr⋅port_dr))"
+definition aBPReceiverIn_stream_dr :: "('e\<times>bool) tsyn stream \<rightarrow> ('e::countable) abpMessage tsyn SB" where
+"aBPReceiverIn_stream_dr = (\<Lambda>  port_dr. (aBP_stream_mediumSr_as__receiver_dr\<cdot>port_dr))"
 
 (* Create one SB for all output channels *)
-definition aBPReceiverOut_stream_ar_o :: "bool tsyn stream → 'e tsyn stream → ('e::countable) abpMessage tsyn SB" where
-"aBPReceiverOut_stream_ar_o = (Λ  port_ar port_o. (aBP_stream_receiver_ar__mediumRs_ar⋅port_ar) ⊎ (aBP_stream_receiver_o__o⋅port_o))"
+definition aBPReceiverOut_stream_ar_o :: "bool tsyn stream \<rightarrow> 'e tsyn stream \<rightarrow> ('e::countable) abpMessage tsyn SB" where
+"aBPReceiverOut_stream_ar_o = (\<Lambda>  port_ar port_o. (aBP_stream_receiver_ar__mediumRs_ar\<cdot>port_ar) \<uplus> (aBP_stream_receiver_o__o\<cdot>port_o))"
 
 
-subsection ‹mediumRs›
+subsection \<open>mediumRs\<close>
 
 (* Create one SB for all input channels *)
-definition aBPMediumRsIn_stream_ar :: "bool tsyn stream → ('e::countable) abpMessage tsyn SB" where
-"aBPMediumRsIn_stream_ar = (Λ  port_ar. (aBP_stream_receiver_ar__mediumRs_ar⋅port_ar))"
+definition aBPMediumRsIn_stream_ar :: "bool tsyn stream \<rightarrow> ('e::countable) abpMessage tsyn SB" where
+"aBPMediumRsIn_stream_ar = (\<Lambda>  port_ar. (aBP_stream_receiver_ar__mediumRs_ar\<cdot>port_ar))"
 
 (* Create one SB for all output channels *)
-definition aBPMediumRsOut_stream_as :: "bool tsyn stream → ('e::countable) abpMessage tsyn SB" where
-"aBPMediumRsOut_stream_as = (Λ  port_as. (aBP_stream_mediumRs_as__sender_as⋅port_as))"
+definition aBPMediumRsOut_stream_as :: "bool tsyn stream \<rightarrow> ('e::countable) abpMessage tsyn SB" where
+"aBPMediumRsOut_stream_as = (\<Lambda>  port_as. (aBP_stream_mediumRs_as__sender_as\<cdot>port_as))"
 
 
-section ‹Helpers to get tsyn elements and streams from sbElems and SBs›
+section \<open>Helpers to get tsyn elements and streams from sbElems and SBs\<close>
 
-definition aBPElem_get_receiver_o__o :: "('e::countable) abpMessage tsyn sbElem ⇒ ('e) tsyn" where
-"aBPElem_get_receiver_o__o sbe = tsynApplyElem (inv DoNotUse_65e4c1937d484f20baf2707bdccbfc49_ABPE) ((Rep_sbElem sbe) ⇀ (𝒞 ''DoNotUse_65e4c1937d484f20baf2707bdccbfc49_receiver_o__o''))"
+definition aBPElem_get_receiver_o__o :: "('e::countable) abpMessage tsyn sbElem \<Rightarrow> ('e) tsyn" where
+"aBPElem_get_receiver_o__o sbe = tsynApplyElem (inv ABPE) ((Rep_sbElem sbe) \<rightharpoonup> (\<C> ''receiver_o__o''))"
 
-lift_definition aBP_get_stream_receiver_o__o :: "('e::countable) abpMessage tsyn SB → 'e tsyn stream" is
-"λsb. tsynMap (inv DoNotUse_65e4c1937d484f20baf2707bdccbfc49_ABPE)⋅(sb . (𝒞 ''DoNotUse_65e4c1937d484f20baf2707bdccbfc49_receiver_o__o''))"
+lift_definition aBP_get_stream_receiver_o__o :: "('e::countable) abpMessage tsyn SB \<rightarrow> 'e tsyn stream" is
+"\<lambda>sb. tsynMap (inv ABPE)\<cdot>(sb . (\<C> ''receiver_o__o''))"
   by(simp add: cfun_def)
 
-definition aBPElem_get_i__sender_i :: "('e::countable) abpMessage tsyn sbElem ⇒ ('e) tsyn" where
-"aBPElem_get_i__sender_i sbe = tsynApplyElem (inv DoNotUse_65e4c1937d484f20baf2707bdccbfc49_ABPE) ((Rep_sbElem sbe) ⇀ (𝒞 ''DoNotUse_65e4c1937d484f20baf2707bdccbfc49_i__sender_i''))"
+definition aBPElem_get_i__sender_i :: "('e::countable) abpMessage tsyn sbElem \<Rightarrow> ('e) tsyn" where
+"aBPElem_get_i__sender_i sbe = tsynApplyElem (inv ABPE) ((Rep_sbElem sbe) \<rightharpoonup> (\<C> ''i__sender_i''))"
 
-lift_definition aBP_get_stream_i__sender_i :: "('e::countable) abpMessage tsyn SB → 'e tsyn stream" is
-"λsb. tsynMap (inv DoNotUse_65e4c1937d484f20baf2707bdccbfc49_ABPE)⋅(sb . (𝒞 ''DoNotUse_65e4c1937d484f20baf2707bdccbfc49_i__sender_i''))"
+lift_definition aBP_get_stream_i__sender_i :: "('e::countable) abpMessage tsyn SB \<rightarrow> 'e tsyn stream" is
+"\<lambda>sb. tsynMap (inv ABPE)\<cdot>(sb . (\<C> ''i__sender_i''))"
   by(simp add: cfun_def)
 
-definition aBPElem_get_sender_ds__mediumSr_ar :: "('e::countable) abpMessage tsyn sbElem ⇒ (('e×bool)) tsyn" where
-"aBPElem_get_sender_ds__mediumSr_ar sbe = tsynApplyElem (inv DoNotUse_65e4c1937d484f20baf2707bdccbfc49_ABPPair_E_Bool) ((Rep_sbElem sbe) ⇀ (𝒞 ''DoNotUse_65e4c1937d484f20baf2707bdccbfc49_sender_ds__mediumSr_ar''))"
+definition aBPElem_get_sender_ds__mediumSr_ar :: "('e::countable) abpMessage tsyn sbElem \<Rightarrow> (('e\<times>bool)) tsyn" where
+"aBPElem_get_sender_ds__mediumSr_ar sbe = tsynApplyElem (inv ABPPair_E_Bool) ((Rep_sbElem sbe) \<rightharpoonup> (\<C> ''sender_ds__mediumSr_ar''))"
 
-lift_definition aBP_get_stream_sender_ds__mediumSr_ar :: "('e::countable) abpMessage tsyn SB → ('e×bool) tsyn stream" is
-"λsb. tsynMap (inv DoNotUse_65e4c1937d484f20baf2707bdccbfc49_ABPPair_E_Bool)⋅(sb . (𝒞 ''DoNotUse_65e4c1937d484f20baf2707bdccbfc49_sender_ds__mediumSr_ar''))"
+lift_definition aBP_get_stream_sender_ds__mediumSr_ar :: "('e::countable) abpMessage tsyn SB \<rightarrow> ('e\<times>bool) tsyn stream" is
+"\<lambda>sb. tsynMap (inv ABPPair_E_Bool)\<cdot>(sb . (\<C> ''sender_ds__mediumSr_ar''))"
   by(simp add: cfun_def)
 
-definition aBPElem_get_mediumSr_as__receiver_dr :: "('e::countable) abpMessage tsyn sbElem ⇒ (('e×bool)) tsyn" where
-"aBPElem_get_mediumSr_as__receiver_dr sbe = tsynApplyElem (inv DoNotUse_65e4c1937d484f20baf2707bdccbfc49_ABPPair_E_Bool) ((Rep_sbElem sbe) ⇀ (𝒞 ''DoNotUse_65e4c1937d484f20baf2707bdccbfc49_mediumSr_as__receiver_dr''))"
+definition aBPElem_get_mediumSr_as__receiver_dr :: "('e::countable) abpMessage tsyn sbElem \<Rightarrow> (('e\<times>bool)) tsyn" where
+"aBPElem_get_mediumSr_as__receiver_dr sbe = tsynApplyElem (inv ABPPair_E_Bool) ((Rep_sbElem sbe) \<rightharpoonup> (\<C> ''mediumSr_as__receiver_dr''))"
 
-lift_definition aBP_get_stream_mediumSr_as__receiver_dr :: "('e::countable) abpMessage tsyn SB → ('e×bool) tsyn stream" is
-"λsb. tsynMap (inv DoNotUse_65e4c1937d484f20baf2707bdccbfc49_ABPPair_E_Bool)⋅(sb . (𝒞 ''DoNotUse_65e4c1937d484f20baf2707bdccbfc49_mediumSr_as__receiver_dr''))"
+lift_definition aBP_get_stream_mediumSr_as__receiver_dr :: "('e::countable) abpMessage tsyn SB \<rightarrow> ('e\<times>bool) tsyn stream" is
+"\<lambda>sb. tsynMap (inv ABPPair_E_Bool)\<cdot>(sb . (\<C> ''mediumSr_as__receiver_dr''))"
   by(simp add: cfun_def)
 
-definition aBPElem_get_receiver_ar__mediumRs_ar :: "('e::countable) abpMessage tsyn sbElem ⇒ (bool) tsyn" where
-"aBPElem_get_receiver_ar__mediumRs_ar sbe = tsynApplyElem (inv DoNotUse_65e4c1937d484f20baf2707bdccbfc49_ABPBool) ((Rep_sbElem sbe) ⇀ (𝒞 ''DoNotUse_65e4c1937d484f20baf2707bdccbfc49_receiver_ar__mediumRs_ar''))"
+definition aBPElem_get_receiver_ar__mediumRs_ar :: "('e::countable) abpMessage tsyn sbElem \<Rightarrow> (bool) tsyn" where
+"aBPElem_get_receiver_ar__mediumRs_ar sbe = tsynApplyElem (inv ABPBool) ((Rep_sbElem sbe) \<rightharpoonup> (\<C> ''receiver_ar__mediumRs_ar''))"
 
-lift_definition aBP_get_stream_receiver_ar__mediumRs_ar :: "('e::countable) abpMessage tsyn SB → bool tsyn stream" is
-"λsb. tsynMap (inv DoNotUse_65e4c1937d484f20baf2707bdccbfc49_ABPBool)⋅(sb . (𝒞 ''DoNotUse_65e4c1937d484f20baf2707bdccbfc49_receiver_ar__mediumRs_ar''))"
+lift_definition aBP_get_stream_receiver_ar__mediumRs_ar :: "('e::countable) abpMessage tsyn SB \<rightarrow> bool tsyn stream" is
+"\<lambda>sb. tsynMap (inv ABPBool)\<cdot>(sb . (\<C> ''receiver_ar__mediumRs_ar''))"
   by(simp add: cfun_def)
 
-definition aBPElem_get_mediumRs_as__sender_as :: "('e::countable) abpMessage tsyn sbElem ⇒ (bool) tsyn" where
-"aBPElem_get_mediumRs_as__sender_as sbe = tsynApplyElem (inv DoNotUse_65e4c1937d484f20baf2707bdccbfc49_ABPBool) ((Rep_sbElem sbe) ⇀ (𝒞 ''DoNotUse_65e4c1937d484f20baf2707bdccbfc49_mediumRs_as__sender_as''))"
+definition aBPElem_get_mediumRs_as__sender_as :: "('e::countable) abpMessage tsyn sbElem \<Rightarrow> (bool) tsyn" where
+"aBPElem_get_mediumRs_as__sender_as sbe = tsynApplyElem (inv ABPBool) ((Rep_sbElem sbe) \<rightharpoonup> (\<C> ''mediumRs_as__sender_as''))"
 
-lift_definition aBP_get_stream_mediumRs_as__sender_as :: "('e::countable) abpMessage tsyn SB → bool tsyn stream" is
-"λsb. tsynMap (inv DoNotUse_65e4c1937d484f20baf2707bdccbfc49_ABPBool)⋅(sb . (𝒞 ''DoNotUse_65e4c1937d484f20baf2707bdccbfc49_mediumRs_as__sender_as''))"
+lift_definition aBP_get_stream_mediumRs_as__sender_as :: "('e::countable) abpMessage tsyn SB \<rightarrow> bool tsyn stream" is
+"\<lambda>sb. tsynMap (inv ABPBool)\<cdot>(sb . (\<C> ''mediumRs_as__sender_as''))"
   by(simp add: cfun_def)
 
 
-section ‹Converter›
+section \<open>Converter\<close>
 
 
-subsection ‹sender›
+subsection \<open>sender\<close>
 
-lift_definition senderInConvert :: "('e::countable) abpMessage tsyn SB → ('e) senderMessage tsyn SB" is
-"λsb. senderIn_stream_as_i⋅(aBP_get_stream_mediumRs_as__sender_as⋅sb)⋅(aBP_get_stream_i__sender_i⋅sb)"
+lift_definition senderInConvert :: "('e::countable) abpMessage tsyn SB \<rightarrow> ('e) senderMessage tsyn SB" is
+"\<lambda>sb. senderIn_stream_as_i\<cdot>(aBP_get_stream_mediumRs_as__sender_as\<cdot>sb)\<cdot>(aBP_get_stream_i__sender_i\<cdot>sb)"
   by (simp add: cfun_def)
 
-lift_definition senderOutConvert :: "('e) senderMessage tsyn SB → ('e::countable) abpMessage tsyn SB" is
-"λsb. aBPSenderOut_stream_ds⋅(sender_get_stream_ds⋅sb)"
+lift_definition senderOutConvert :: "('e) senderMessage tsyn SB \<rightarrow> ('e::countable) abpMessage tsyn SB" is
+"\<lambda>sb. aBPSenderOut_stream_ds\<cdot>(sender_get_stream_ds\<cdot>sb)"
   by (simp add: cfun_def)
 
-definition senderInConverterSPF :: "('e::countable) abpMessage tsyn SB ⇛ ('e) senderMessage tsyn SB" where
+definition senderInConverterSPF :: "('e::countable) abpMessage tsyn SB \<Rrightarrow> ('e) senderMessage tsyn SB" where
 "senderInConverterSPF = ufLift aBPSenderDom senderInConvert"
 
-definition senderOutConverterSPF :: "('e) senderMessage tsyn SB ⇛ ('e::countable) abpMessage tsyn SB" where
+definition senderOutConverterSPF :: "('e) senderMessage tsyn SB \<Rrightarrow> ('e::countable) abpMessage tsyn SB" where
 "senderOutConverterSPF = ufLift aBPSenderRan senderOutConvert"
 
 
-subsection ‹mediumSr›
+subsection \<open>mediumSr\<close>
 
-lift_definition mediumSrInConvert :: "('e::countable) abpMessage tsyn SB → (('e×bool)) mediumMessage tsyn SB" is
-"λsb. mediumIn_stream_ar⋅(aBP_get_stream_sender_ds__mediumSr_ar⋅sb)"
+lift_definition mediumSrInConvert :: "('e::countable) abpMessage tsyn SB \<rightarrow> (('e\<times>bool)) mediumMessage tsyn SB" is
+"\<lambda>sb. mediumIn_stream_ar\<cdot>(aBP_get_stream_sender_ds__mediumSr_ar\<cdot>sb)"
   by (simp add: cfun_def)
 
-lift_definition mediumSrOutConvert :: "(('e×bool)) mediumMessage tsyn SB → ('e::countable) abpMessage tsyn SB" is
-"λsb. aBPMediumSrOut_stream_as⋅(medium_get_stream_as⋅sb)"
+lift_definition mediumSrOutConvert :: "(('e\<times>bool)) mediumMessage tsyn SB \<rightarrow> ('e::countable) abpMessage tsyn SB" is
+"\<lambda>sb. aBPMediumSrOut_stream_as\<cdot>(medium_get_stream_as\<cdot>sb)"
   by (simp add: cfun_def)
 
-definition mediumSrInConverterSPF :: "('e::countable) abpMessage tsyn SB ⇛ (('e×bool)) mediumMessage tsyn SB" where
+definition mediumSrInConverterSPF :: "('e::countable) abpMessage tsyn SB \<Rrightarrow> (('e\<times>bool)) mediumMessage tsyn SB" where
 "mediumSrInConverterSPF = ufLift aBPMediumSrDom mediumSrInConvert"
 
-definition mediumSrOutConverterSPF :: "(('e×bool)) mediumMessage tsyn SB ⇛ ('e::countable) abpMessage tsyn SB" where
+definition mediumSrOutConverterSPF :: "(('e\<times>bool)) mediumMessage tsyn SB \<Rrightarrow> ('e::countable) abpMessage tsyn SB" where
 "mediumSrOutConverterSPF = ufLift aBPMediumSrRan mediumSrOutConvert"
 
 
-subsection ‹receiver›
+subsection \<open>receiver\<close>
 
-lift_definition receiverInConvert :: "('e::countable) abpMessage tsyn SB → ('e) receiverMessage tsyn SB" is
-"λsb. receiverIn_stream_dr⋅(aBP_get_stream_mediumSr_as__receiver_dr⋅sb)"
+lift_definition receiverInConvert :: "('e::countable) abpMessage tsyn SB \<rightarrow> ('e) receiverMessage tsyn SB" is
+"\<lambda>sb. receiverIn_stream_dr\<cdot>(aBP_get_stream_mediumSr_as__receiver_dr\<cdot>sb)"
   by (simp add: cfun_def)
 
-lift_definition receiverOutConvert :: "('e) receiverMessage tsyn SB → ('e::countable) abpMessage tsyn SB" is
-"λsb. aBPReceiverOut_stream_ar_o⋅(receiver_get_stream_ar⋅sb)⋅(receiver_get_stream_o⋅sb)"
+lift_definition receiverOutConvert :: "('e) receiverMessage tsyn SB \<rightarrow> ('e::countable) abpMessage tsyn SB" is
+"\<lambda>sb. aBPReceiverOut_stream_ar_o\<cdot>(receiver_get_stream_ar\<cdot>sb)\<cdot>(receiver_get_stream_o\<cdot>sb)"
   by (simp add: cfun_def)
 
-definition receiverInConverterSPF :: "('e::countable) abpMessage tsyn SB ⇛ ('e) receiverMessage tsyn SB" where
+definition receiverInConverterSPF :: "('e::countable) abpMessage tsyn SB \<Rrightarrow> ('e) receiverMessage tsyn SB" where
 "receiverInConverterSPF = ufLift aBPReceiverDom receiverInConvert"
 
-definition receiverOutConverterSPF :: "('e) receiverMessage tsyn SB ⇛ ('e::countable) abpMessage tsyn SB" where
+definition receiverOutConverterSPF :: "('e) receiverMessage tsyn SB \<Rrightarrow> ('e::countable) abpMessage tsyn SB" where
 "receiverOutConverterSPF = ufLift aBPReceiverRan receiverOutConvert"
 
 
-subsection ‹mediumRs›
+subsection \<open>mediumRs\<close>
 
-lift_definition mediumRsInConvert :: "('e::countable) abpMessage tsyn SB → (bool) mediumMessage tsyn SB" is
-"λsb. mediumIn_stream_ar⋅(aBP_get_stream_receiver_ar__mediumRs_ar⋅sb)"
+lift_definition mediumRsInConvert :: "('e::countable) abpMessage tsyn SB \<rightarrow> (bool) mediumMessage tsyn SB" is
+"\<lambda>sb. mediumIn_stream_ar\<cdot>(aBP_get_stream_receiver_ar__mediumRs_ar\<cdot>sb)"
   by (simp add: cfun_def)
 
-lift_definition mediumRsOutConvert :: "(bool) mediumMessage tsyn SB → ('e::countable) abpMessage tsyn SB" is
-"λsb. aBPMediumRsOut_stream_as⋅(medium_get_stream_as⋅sb)"
+lift_definition mediumRsOutConvert :: "(bool) mediumMessage tsyn SB \<rightarrow> ('e::countable) abpMessage tsyn SB" is
+"\<lambda>sb. aBPMediumRsOut_stream_as\<cdot>(medium_get_stream_as\<cdot>sb)"
   by (simp add: cfun_def)
 
-definition mediumRsInConverterSPF :: "('e::countable) abpMessage tsyn SB ⇛ (bool) mediumMessage tsyn SB" where
+definition mediumRsInConverterSPF :: "('e::countable) abpMessage tsyn SB \<Rrightarrow> (bool) mediumMessage tsyn SB" where
 "mediumRsInConverterSPF = ufLift aBPMediumRsDom mediumRsInConvert"
 
-definition mediumRsOutConverterSPF :: "(bool) mediumMessage tsyn SB ⇛ ('e::countable) abpMessage tsyn SB" where
+definition mediumRsOutConverterSPF :: "(bool) mediumMessage tsyn SB \<Rrightarrow> ('e::countable) abpMessage tsyn SB" where
 "mediumRsOutConverterSPF = ufLift aBPMediumRsRan mediumRsOutConvert"
 
 
-section ‹Instances›
+section \<open>Instances\<close>
 
 definition aBPSender :: "(('e::countable) abpMessage tsyn, ('e::countable) abpMessage tsyn) SPF" where
-"aBPSender = (senderInConverterSPF∘senderSPF∘senderOutConverterSPF)"
+"aBPSender = (senderInConverterSPF\<circ>senderSPF\<circ>senderOutConverterSPF)"
 
 definition aBPMediumSr :: "('e::countable) abpMessage tsyn SPS" where
-"aBPMediumSr = ((uspecConst mediumSrInConverterSPF)○mediumSPS○(uspecConst mediumSrOutConverterSPF))"
+"aBPMediumSr = ((uspecConst mediumSrInConverterSPF)\<circle>mediumSPS\<circle>(uspecConst mediumSrOutConverterSPF))"
 
 definition aBPReceiver :: "(('e::countable) abpMessage tsyn, ('e::countable) abpMessage tsyn) SPF" where
-"aBPReceiver = (receiverInConverterSPF∘receiverSPF∘receiverOutConverterSPF)"
+"aBPReceiver = (receiverInConverterSPF\<circ>receiverSPF\<circ>receiverOutConverterSPF)"
 
 definition aBPMediumRs :: "('e::countable) abpMessage tsyn SPS" where
-"aBPMediumRs = ((uspecConst mediumRsInConverterSPF)○mediumSPS○(uspecConst mediumRsOutConverterSPF))"
+"aBPMediumRs = ((uspecConst mediumRsInConverterSPF)\<circle>mediumSPS\<circle>(uspecConst mediumRsOutConverterSPF))"
 
 
-section ‹Final definition›
+section \<open>Final definition\<close>
 
 definition aBPSPS :: "('e::countable) abpMessage tsyn SPS" where
-"aBPSPS = ((uspecConst aBPSender)⨂aBPMediumSr⨂(uspecConst aBPReceiver)⨂aBPMediumRs)"
+"aBPSPS = ((uspecConst aBPSender)\<Otimes>aBPMediumSr\<Otimes>(uspecConst aBPReceiver)\<Otimes>aBPMediumRs)"
 
 
-section ‹Lemmas for single tsyn setter›
+section \<open>Lemmas for single tsyn setter\<close>
 
-lemma abpelem_receiver_o__o_dom[simp]: "sbeDom (aBPElem_receiver_o__o x) = {𝒞 ''DoNotUse_65e4c1937d484f20baf2707bdccbfc49_receiver_o__o''}"
+lemma abpelem_receiver_o__o_dom[simp]: "sbeDom (aBPElem_receiver_o__o x) = {\<C> ''receiver_o__o''}"
   apply(cases x)
   apply(simp add: aBPElem_receiver_o__o.simps sbeDom_def aBPElem_raw_receiver_o__o.rep_eq)
   by(simp add: aBPElem_receiver_o__o.simps)
 
-lemma abpelem_i__sender_i_dom[simp]: "sbeDom (aBPElem_i__sender_i x) = {𝒞 ''DoNotUse_65e4c1937d484f20baf2707bdccbfc49_i__sender_i''}"
+lemma abpelem_i__sender_i_dom[simp]: "sbeDom (aBPElem_i__sender_i x) = {\<C> ''i__sender_i''}"
   apply(cases x)
   apply(simp add: aBPElem_i__sender_i.simps sbeDom_def aBPElem_raw_i__sender_i.rep_eq)
   by(simp add: aBPElem_i__sender_i.simps)
 
-lemma abpelem_sender_ds__mediumsr_ar_dom[simp]: "sbeDom (aBPElem_sender_ds__mediumSr_ar x) = {𝒞 ''DoNotUse_65e4c1937d484f20baf2707bdccbfc49_sender_ds__mediumSr_ar''}"
+lemma abpelem_sender_ds__mediumsr_ar_dom[simp]: "sbeDom (aBPElem_sender_ds__mediumSr_ar x) = {\<C> ''sender_ds__mediumSr_ar''}"
   apply(cases x)
   apply(simp add: aBPElem_sender_ds__mediumSr_ar.simps sbeDom_def aBPElem_raw_sender_ds__mediumSr_ar.rep_eq)
   by(simp add: aBPElem_sender_ds__mediumSr_ar.simps)
 
-lemma abpelem_mediumsr_as__receiver_dr_dom[simp]: "sbeDom (aBPElem_mediumSr_as__receiver_dr x) = {𝒞 ''DoNotUse_65e4c1937d484f20baf2707bdccbfc49_mediumSr_as__receiver_dr''}"
+lemma abpelem_mediumsr_as__receiver_dr_dom[simp]: "sbeDom (aBPElem_mediumSr_as__receiver_dr x) = {\<C> ''mediumSr_as__receiver_dr''}"
   apply(cases x)
   apply(simp add: aBPElem_mediumSr_as__receiver_dr.simps sbeDom_def aBPElem_raw_mediumSr_as__receiver_dr.rep_eq)
   by(simp add: aBPElem_mediumSr_as__receiver_dr.simps)
 
-lemma abpelem_receiver_ar__mediumrs_ar_dom[simp]: "sbeDom (aBPElem_receiver_ar__mediumRs_ar x) = {𝒞 ''DoNotUse_65e4c1937d484f20baf2707bdccbfc49_receiver_ar__mediumRs_ar''}"
+lemma abpelem_receiver_ar__mediumrs_ar_dom[simp]: "sbeDom (aBPElem_receiver_ar__mediumRs_ar x) = {\<C> ''receiver_ar__mediumRs_ar''}"
   apply(cases x)
   apply(simp add: aBPElem_receiver_ar__mediumRs_ar.simps sbeDom_def aBPElem_raw_receiver_ar__mediumRs_ar.rep_eq)
   by(simp add: aBPElem_receiver_ar__mediumRs_ar.simps)
 
-lemma abpelem_mediumrs_as__sender_as_dom[simp]: "sbeDom (aBPElem_mediumRs_as__sender_as x) = {𝒞 ''DoNotUse_65e4c1937d484f20baf2707bdccbfc49_mediumRs_as__sender_as''}"
+lemma abpelem_mediumrs_as__sender_as_dom[simp]: "sbeDom (aBPElem_mediumRs_as__sender_as x) = {\<C> ''mediumRs_as__sender_as''}"
   apply(cases x)
   apply(simp add: aBPElem_mediumRs_as__sender_as.simps sbeDom_def aBPElem_raw_mediumRs_as__sender_as.rep_eq)
   by(simp add: aBPElem_mediumRs_as__sender_as.simps)
@@ -707,14 +707,14 @@ lemma abpelemin_i_dom[simp]: "sbeDom (aBPElemIn_i port_i) = aBPDom"
 lemma abpelemout_o_dom[simp]: "sbeDom (aBPElemOut_o port_o) = aBPRan"
   by(auto simp add: aBPElemOut_o_def aBPRan_def)
 
-lemma abpin_i_dom[simp]: "ubDom⋅(aBPIn_i port_i) = aBPDom"
+lemma abpin_i_dom[simp]: "ubDom\<cdot>(aBPIn_i port_i) = aBPDom"
   by(simp add: aBPIn_i_def)
 
-lemma abpout_o_dom[simp]: "ubDom⋅(aBPOut_o port_o) = aBPRan"
+lemma abpout_o_dom[simp]: "ubDom\<cdot>(aBPOut_o port_o) = aBPRan"
   by(simp add: aBPOut_o_def)
 
 
-subsection ‹sender›
+subsection \<open>sender\<close>
 
 lemma abpsenderelemin_as_i_dom[simp]: "sbeDom (aBPSenderElemIn_as_i port_as port_i) = aBPSenderDom"
   sorry
@@ -722,14 +722,14 @@ lemma abpsenderelemin_as_i_dom[simp]: "sbeDom (aBPSenderElemIn_as_i port_as port
 lemma abpsenderelemout_ds_dom[simp]: "sbeDom (aBPSenderElemOut_ds port_ds) = aBPSenderRan"
   sorry
 
-lemma abpsenderin_as_i_dom[simp]: "ubDom⋅(aBPSenderIn_as_i port_as port_i) = aBPSenderDom"
+lemma abpsenderin_as_i_dom[simp]: "ubDom\<cdot>(aBPSenderIn_as_i port_as port_i) = aBPSenderDom"
   sorry
 
-lemma abpsenderout_ds_dom[simp]: "ubDom⋅(aBPSenderOut_ds port_ds) = aBPSenderRan"
+lemma abpsenderout_ds_dom[simp]: "ubDom\<cdot>(aBPSenderOut_ds port_ds) = aBPSenderRan"
   sorry
 
 
-subsection ‹mediumSr›
+subsection \<open>mediumSr\<close>
 
 lemma abpmediumsrelemin_ar_dom[simp]: "sbeDom (aBPMediumSrElemIn_ar port_ar) = aBPMediumSrDom"
   sorry
@@ -737,14 +737,14 @@ lemma abpmediumsrelemin_ar_dom[simp]: "sbeDom (aBPMediumSrElemIn_ar port_ar) = a
 lemma abpmediumsrelemout_as_dom[simp]: "sbeDom (aBPMediumSrElemOut_as port_as) = aBPMediumSrRan"
   sorry
 
-lemma abpmediumsrin_ar_dom[simp]: "ubDom⋅(aBPMediumSrIn_ar port_ar) = aBPMediumSrDom"
+lemma abpmediumsrin_ar_dom[simp]: "ubDom\<cdot>(aBPMediumSrIn_ar port_ar) = aBPMediumSrDom"
   sorry
 
-lemma abpmediumsrout_as_dom[simp]: "ubDom⋅(aBPMediumSrOut_as port_as) = aBPMediumSrRan"
+lemma abpmediumsrout_as_dom[simp]: "ubDom\<cdot>(aBPMediumSrOut_as port_as) = aBPMediumSrRan"
   sorry
 
 
-subsection ‹receiver›
+subsection \<open>receiver\<close>
 
 lemma abpreceiverelemin_dr_dom[simp]: "sbeDom (aBPReceiverElemIn_dr port_dr) = aBPReceiverDom"
   sorry
@@ -752,14 +752,14 @@ lemma abpreceiverelemin_dr_dom[simp]: "sbeDom (aBPReceiverElemIn_dr port_dr) = a
 lemma abpreceiverelemout_ar_o_dom[simp]: "sbeDom (aBPReceiverElemOut_ar_o port_ar port_o) = aBPReceiverRan"
   sorry
 
-lemma abpreceiverin_dr_dom[simp]: "ubDom⋅(aBPReceiverIn_dr port_dr) = aBPReceiverDom"
+lemma abpreceiverin_dr_dom[simp]: "ubDom\<cdot>(aBPReceiverIn_dr port_dr) = aBPReceiverDom"
   sorry
 
-lemma abpreceiverout_ar_o_dom[simp]: "ubDom⋅(aBPReceiverOut_ar_o port_ar port_o) = aBPReceiverRan"
+lemma abpreceiverout_ar_o_dom[simp]: "ubDom\<cdot>(aBPReceiverOut_ar_o port_ar port_o) = aBPReceiverRan"
   sorry
 
 
-subsection ‹mediumRs›
+subsection \<open>mediumRs\<close>
 
 lemma abpmediumrselemin_ar_dom[simp]: "sbeDom (aBPMediumRsElemIn_ar port_ar) = aBPMediumRsDom"
   sorry
@@ -767,37 +767,89 @@ lemma abpmediumrselemin_ar_dom[simp]: "sbeDom (aBPMediumRsElemIn_ar port_ar) = a
 lemma abpmediumrselemout_as_dom[simp]: "sbeDom (aBPMediumRsElemOut_as port_as) = aBPMediumRsRan"
   sorry
 
-lemma abpmediumrsin_ar_dom[simp]: "ubDom⋅(aBPMediumRsIn_ar port_ar) = aBPMediumRsDom"
+lemma abpmediumrsin_ar_dom[simp]: "ubDom\<cdot>(aBPMediumRsIn_ar port_ar) = aBPMediumRsDom"
   sorry
 
-lemma abpmediumrsout_as_dom[simp]: "ubDom⋅(aBPMediumRsOut_as port_as) = aBPMediumRsRan"
+lemma abpmediumrsout_as_dom[simp]: "ubDom\<cdot>(aBPMediumRsOut_as port_as) = aBPMediumRsRan"
   sorry
 
 
-section ‹stream-setter (just for simp)›
+section \<open>Stream-setter\<close>
 
-lemma [simp]: "ubDom⋅(aBP_stream_receiver_o__o⋅x) = {𝒞 ''DoNotUse_65e4c1937d484f20baf2707bdccbfc49_receiver_o__o''}"
-  by(simp add: aBP_stream_receiver_o__o.rep_eq ubdom_insert DoNotUse_65e4c1937d484f20baf2707bdccbfc49_aBP_stream_receiver_o__o_h.rep_eq)
+lemma abp_stream_receiver_o__o_dom[simp]: "ubDom\<cdot>(aBP_stream_receiver_o__o\<cdot>x) = {\<C> ''receiver_o__o''}"
+  by(simp add: aBP_stream_receiver_o__o.rep_eq ubdom_insert aBP_stream_receiver_o__o_h.rep_eq)
 
-lemma [simp]: "ubDom⋅(aBP_stream_i__sender_i⋅x) = {𝒞 ''DoNotUse_65e4c1937d484f20baf2707bdccbfc49_i__sender_i''}"
-  by(simp add: aBP_stream_i__sender_i.rep_eq ubdom_insert DoNotUse_65e4c1937d484f20baf2707bdccbfc49_aBP_stream_i__sender_i_h.rep_eq)
+lemma abp_stream_i__sender_i_dom[simp]: "ubDom\<cdot>(aBP_stream_i__sender_i\<cdot>x) = {\<C> ''i__sender_i''}"
+  by(simp add: aBP_stream_i__sender_i.rep_eq ubdom_insert aBP_stream_i__sender_i_h.rep_eq)
 
-lemma [simp]: "ubDom⋅(aBP_stream_sender_ds__mediumSr_ar⋅x) = {𝒞 ''DoNotUse_65e4c1937d484f20baf2707bdccbfc49_sender_ds__mediumSr_ar''}"
-  by(simp add: aBP_stream_sender_ds__mediumSr_ar.rep_eq ubdom_insert DoNotUse_65e4c1937d484f20baf2707bdccbfc49_aBP_stream_sender_ds__mediumSr_ar_h.rep_eq)
+lemma abp_stream_sender_ds__mediumsr_ar_dom[simp]: "ubDom\<cdot>(aBP_stream_sender_ds__mediumSr_ar\<cdot>x) = {\<C> ''sender_ds__mediumSr_ar''}"
+  by(simp add: aBP_stream_sender_ds__mediumSr_ar.rep_eq ubdom_insert aBP_stream_sender_ds__mediumSr_ar_h.rep_eq)
 
-lemma [simp]: "ubDom⋅(aBP_stream_mediumSr_as__receiver_dr⋅x) = {𝒞 ''DoNotUse_65e4c1937d484f20baf2707bdccbfc49_mediumSr_as__receiver_dr''}"
-  by(simp add: aBP_stream_mediumSr_as__receiver_dr.rep_eq ubdom_insert DoNotUse_65e4c1937d484f20baf2707bdccbfc49_aBP_stream_mediumSr_as__receiver_dr_h.rep_eq)
+lemma abp_stream_mediumsr_as__receiver_dr_dom[simp]: "ubDom\<cdot>(aBP_stream_mediumSr_as__receiver_dr\<cdot>x) = {\<C> ''mediumSr_as__receiver_dr''}"
+  by(simp add: aBP_stream_mediumSr_as__receiver_dr.rep_eq ubdom_insert aBP_stream_mediumSr_as__receiver_dr_h.rep_eq)
 
-lemma [simp]: "ubDom⋅(aBP_stream_receiver_ar__mediumRs_ar⋅x) = {𝒞 ''DoNotUse_65e4c1937d484f20baf2707bdccbfc49_receiver_ar__mediumRs_ar''}"
-  by(simp add: aBP_stream_receiver_ar__mediumRs_ar.rep_eq ubdom_insert DoNotUse_65e4c1937d484f20baf2707bdccbfc49_aBP_stream_receiver_ar__mediumRs_ar_h.rep_eq)
+lemma abp_stream_receiver_ar__mediumrs_ar_dom[simp]: "ubDom\<cdot>(aBP_stream_receiver_ar__mediumRs_ar\<cdot>x) = {\<C> ''receiver_ar__mediumRs_ar''}"
+  by(simp add: aBP_stream_receiver_ar__mediumRs_ar.rep_eq ubdom_insert aBP_stream_receiver_ar__mediumRs_ar_h.rep_eq)
 
-lemma [simp]: "ubDom⋅(aBP_stream_mediumRs_as__sender_as⋅x) = {𝒞 ''DoNotUse_65e4c1937d484f20baf2707bdccbfc49_mediumRs_as__sender_as''}"
-  by(simp add: aBP_stream_mediumRs_as__sender_as.rep_eq ubdom_insert DoNotUse_65e4c1937d484f20baf2707bdccbfc49_aBP_stream_mediumRs_as__sender_as_h.rep_eq)
+lemma abp_stream_mediumrs_as__sender_as_dom[simp]: "ubDom\<cdot>(aBP_stream_mediumRs_as__sender_as\<cdot>x) = {\<C> ''mediumRs_as__sender_as''}"
+  by(simp add: aBP_stream_mediumRs_as__sender_as.rep_eq ubdom_insert aBP_stream_mediumRs_as__sender_as_h.rep_eq)
+
+lemma abpin_stream_i_dom[simp]: "ubDom\<cdot>(aBPIn_stream_i\<cdot>port_i__sender_port_i) = aBPDom"
+  apply(simp add: aBPIn_stream_i_def ubclUnion_ubundle_def)
+  by(auto simp add: aBPDom_def)
+
+lemma abpout_stream_o_dom[simp]: "ubDom\<cdot>(aBPOut_stream_o\<cdot>receiver_port_o__port_o) = aBPRan"
+  apply(simp add: aBPOut_stream_o_def ubclUnion_ubundle_def)
+  by(auto simp add: aBPRan_def)
 
 
-section ‹Lemmas for getter›
+subsection \<open>sender\<close>
 
-subsection ‹Identity lemmas for single sbElems›
+lemma abpsenderin_stream_as_i_dom[simp]: "ubDom\<cdot>(aBPSenderIn_stream_as_i\<cdot>    mediumRs_port_as__sender_port_as\<cdot>port_i__sender_port_i) = aBPSenderDom"
+  apply(simp add: aBPSenderIn_stream_as_i_def ubclUnion_ubundle_def)
+  by(auto simp add: aBPSenderDom_def)
+
+lemma abpsenderout_stream_ds_dom[simp]: "ubDom\<cdot>(aBPSenderOut_stream_ds\<cdot>    sender_port_ds__mediumSr_port_ar) = aBPSenderRan"
+  apply(simp add: aBPSenderOut_stream_ds_def ubclUnion_ubundle_def)
+  by(auto simp add: aBPSenderRan_def)
+
+
+subsection \<open>mediumSr\<close>
+
+lemma abpmediumsrin_stream_ar_dom[simp]: "ubDom\<cdot>(aBPMediumSrIn_stream_ar\<cdot>    sender_port_ds__mediumSr_port_ar) = aBPMediumSrDom"
+  apply(simp add: aBPMediumSrIn_stream_ar_def ubclUnion_ubundle_def)
+  by(auto simp add: aBPMediumSrDom_def)
+
+lemma abpmediumsrout_stream_as_dom[simp]: "ubDom\<cdot>(aBPMediumSrOut_stream_as\<cdot>    mediumSr_port_as__receiver_port_dr) = aBPMediumSrRan"
+  apply(simp add: aBPMediumSrOut_stream_as_def ubclUnion_ubundle_def)
+  by(auto simp add: aBPMediumSrRan_def)
+
+
+subsection \<open>receiver\<close>
+
+lemma abpreceiverin_stream_dr_dom[simp]: "ubDom\<cdot>(aBPReceiverIn_stream_dr\<cdot>    mediumSr_port_as__receiver_port_dr) = aBPReceiverDom"
+  apply(simp add: aBPReceiverIn_stream_dr_def ubclUnion_ubundle_def)
+  by(auto simp add: aBPReceiverDom_def)
+
+lemma abpreceiverout_stream_ar_o_dom[simp]: "ubDom\<cdot>(aBPReceiverOut_stream_ar_o\<cdot>    receiver_port_ar__mediumRs_port_ar\<cdot>receiver_port_o__port_o) = aBPReceiverRan"
+  apply(simp add: aBPReceiverOut_stream_ar_o_def ubclUnion_ubundle_def)
+  by(auto simp add: aBPReceiverRan_def)
+
+
+subsection \<open>mediumRs\<close>
+
+lemma abpmediumrsin_stream_ar_dom[simp]: "ubDom\<cdot>(aBPMediumRsIn_stream_ar\<cdot>    receiver_port_ar__mediumRs_port_ar) = aBPMediumRsDom"
+  apply(simp add: aBPMediumRsIn_stream_ar_def ubclUnion_ubundle_def)
+  by(auto simp add: aBPMediumRsDom_def)
+
+lemma abpmediumrsout_stream_as_dom[simp]: "ubDom\<cdot>(aBPMediumRsOut_stream_as\<cdot>    mediumRs_port_as__sender_port_as) = aBPMediumRsRan"
+  apply(simp add: aBPMediumRsOut_stream_as_def ubclUnion_ubundle_def)
+  by(auto simp add: aBPMediumRsRan_def)
+
+
+section \<open>Lemmas for getter\<close>
+
+subsection \<open>Identity lemmas for single sbElems\<close>
 
 lemma abpelem_receiver_o__o_id[simp]: "aBPElem_get_receiver_o__o (aBPElem_receiver_o__o x) = x"
   apply(cases x)
@@ -848,56 +900,56 @@ lemma abpelem_mediumrs_as__sender_as_id[simp]: "aBPElem_get_mediumRs_as__sender_
   by(simp add: sbeNull.rep_eq)
 
 
-subsection ‹Identity lemmas for single SBs from streams›
+subsection \<open>Identity lemmas for single SBs from streams\<close>
 
-lemma abp_stream_receiver_o__o_id[simp]: "aBP_get_stream_receiver_o__o⋅(aBP_stream_receiver_o__o⋅x) = x"
+lemma abp_stream_receiver_o__o_id[simp]: "aBP_get_stream_receiver_o__o\<cdot>(aBP_stream_receiver_o__o\<cdot>x) = x"
   apply(simp add: aBP_get_stream_receiver_o__o.rep_eq aBP_stream_receiver_o__o.rep_eq)
-  apply(simp add: ubGetCh_def DoNotUse_65e4c1937d484f20baf2707bdccbfc49_aBP_stream_receiver_o__o_h.rep_eq)
+  apply(simp add: ubGetCh_def aBP_stream_receiver_o__o_h.rep_eq)
   by (simp add: inj_def)
 
-lemma abp_stream_i__sender_i_id[simp]: "aBP_get_stream_i__sender_i⋅(aBP_stream_i__sender_i⋅x) = x"
+lemma abp_stream_i__sender_i_id[simp]: "aBP_get_stream_i__sender_i\<cdot>(aBP_stream_i__sender_i\<cdot>x) = x"
   apply(simp add: aBP_get_stream_i__sender_i.rep_eq aBP_stream_i__sender_i.rep_eq)
-  apply(simp add: ubGetCh_def DoNotUse_65e4c1937d484f20baf2707bdccbfc49_aBP_stream_i__sender_i_h.rep_eq)
+  apply(simp add: ubGetCh_def aBP_stream_i__sender_i_h.rep_eq)
   by (simp add: inj_def)
 
-lemma abp_stream_sender_ds__mediumsr_ar_id[simp]: "aBP_get_stream_sender_ds__mediumSr_ar⋅(aBP_stream_sender_ds__mediumSr_ar⋅x) = x"
+lemma abp_stream_sender_ds__mediumsr_ar_id[simp]: "aBP_get_stream_sender_ds__mediumSr_ar\<cdot>(aBP_stream_sender_ds__mediumSr_ar\<cdot>x) = x"
   apply(simp add: aBP_get_stream_sender_ds__mediumSr_ar.rep_eq aBP_stream_sender_ds__mediumSr_ar.rep_eq)
-  apply(simp add: ubGetCh_def DoNotUse_65e4c1937d484f20baf2707bdccbfc49_aBP_stream_sender_ds__mediumSr_ar_h.rep_eq)
+  apply(simp add: ubGetCh_def aBP_stream_sender_ds__mediumSr_ar_h.rep_eq)
   by (simp add: inj_def)
 
-lemma abp_stream_mediumsr_as__receiver_dr_id[simp]: "aBP_get_stream_mediumSr_as__receiver_dr⋅(aBP_stream_mediumSr_as__receiver_dr⋅x) = x"
+lemma abp_stream_mediumsr_as__receiver_dr_id[simp]: "aBP_get_stream_mediumSr_as__receiver_dr\<cdot>(aBP_stream_mediumSr_as__receiver_dr\<cdot>x) = x"
   apply(simp add: aBP_get_stream_mediumSr_as__receiver_dr.rep_eq aBP_stream_mediumSr_as__receiver_dr.rep_eq)
-  apply(simp add: ubGetCh_def DoNotUse_65e4c1937d484f20baf2707bdccbfc49_aBP_stream_mediumSr_as__receiver_dr_h.rep_eq)
+  apply(simp add: ubGetCh_def aBP_stream_mediumSr_as__receiver_dr_h.rep_eq)
   by (simp add: inj_def)
 
-lemma abp_stream_receiver_ar__mediumrs_ar_id[simp]: "aBP_get_stream_receiver_ar__mediumRs_ar⋅(aBP_stream_receiver_ar__mediumRs_ar⋅x) = x"
+lemma abp_stream_receiver_ar__mediumrs_ar_id[simp]: "aBP_get_stream_receiver_ar__mediumRs_ar\<cdot>(aBP_stream_receiver_ar__mediumRs_ar\<cdot>x) = x"
   apply(simp add: aBP_get_stream_receiver_ar__mediumRs_ar.rep_eq aBP_stream_receiver_ar__mediumRs_ar.rep_eq)
-  apply(simp add: ubGetCh_def DoNotUse_65e4c1937d484f20baf2707bdccbfc49_aBP_stream_receiver_ar__mediumRs_ar_h.rep_eq)
+  apply(simp add: ubGetCh_def aBP_stream_receiver_ar__mediumRs_ar_h.rep_eq)
   by (simp add: inj_def)
 
-lemma abp_stream_mediumrs_as__sender_as_id[simp]: "aBP_get_stream_mediumRs_as__sender_as⋅(aBP_stream_mediumRs_as__sender_as⋅x) = x"
+lemma abp_stream_mediumrs_as__sender_as_id[simp]: "aBP_get_stream_mediumRs_as__sender_as\<cdot>(aBP_stream_mediumRs_as__sender_as\<cdot>x) = x"
   apply(simp add: aBP_get_stream_mediumRs_as__sender_as.rep_eq aBP_stream_mediumRs_as__sender_as.rep_eq)
-  apply(simp add: ubGetCh_def DoNotUse_65e4c1937d484f20baf2707bdccbfc49_aBP_stream_mediumRs_as__sender_as_h.rep_eq)
+  apply(simp add: ubGetCh_def aBP_stream_mediumRs_as__sender_as_h.rep_eq)
   by (simp add: inj_def)
 
 
-subsection ‹Identity lemmas for input sbElems›
+subsection \<open>Identity lemmas for input sbElems\<close>
 
 lemma abpelemin_i_i__sender_i_id[simp]: "aBPElem_get_i__sender_i (aBPElemIn_i port_i__sender_port_i) = port_i__sender_port_i"
   apply(simp add: aBPElemIn_i_def aBPElem_get_i__sender_i_def)
   by(metis aBPElem_get_i__sender_i_def abpelem_i__sender_i_id)
 
 
-subsection ‹Identity lemmas for output sbElems›
+subsection \<open>Identity lemmas for output sbElems\<close>
 
 lemma abpelemout_o_receiver_o__o_id[simp]: "aBPElem_get_receiver_o__o (aBPElemOut_o receiver_port_o__port_o) = receiver_port_o__port_o"
   apply(simp add: aBPElemOut_o_def aBPElem_get_receiver_o__o_def)
   by(metis aBPElem_get_receiver_o__o_def abpelem_receiver_o__o_id)
 
 
-subsection ‹Identity lemmas for input SBs›
+subsection \<open>Identity lemmas for input SBs\<close>
 
-lemma abpin_i_i__sender_i_id[simp]: "aBP_get_stream_i__sender_i⋅(aBPIn_i port_i__sender_port_i) = ↑port_i__sender_port_i"
+lemma abpin_i_i__sender_i_id[simp]: "aBP_get_stream_i__sender_i\<cdot>(aBPIn_i port_i__sender_port_i) = \<up>port_i__sender_port_i"
   apply(simp add: aBP_get_stream_i__sender_i_def aBPIn_i_def)
   apply(subst sbe2sb_getch)
   apply(auto simp add: aBPDom_def aBPElemIn_i_def)
@@ -908,9 +960,9 @@ lemma abpin_i_i__sender_i_id[simp]: "aBP_get_stream_i__sender_i⋅(aBPIn_i port_
   by(simp add: sbeNull.rep_eq)
 
 
-subsection ‹Identity lemmas for output SBs›
+subsection \<open>Identity lemmas for output SBs\<close>
 
-lemma abpout_o_receiver_o__o_id[simp]: "aBP_get_stream_receiver_o__o⋅(aBPOut_o receiver_port_o__port_o) = ↑receiver_port_o__port_o"
+lemma abpout_o_receiver_o__o_id[simp]: "aBP_get_stream_receiver_o__o\<cdot>(aBPOut_o receiver_port_o__port_o) = \<up>receiver_port_o__port_o"
   apply(simp add: aBP_get_stream_receiver_o__o_def aBPOut_o_def)
   apply(subst sbe2sb_getch)
   apply(auto simp add: aBPDom_def aBPElemOut_o_def)
@@ -921,16 +973,16 @@ lemma abpout_o_receiver_o__o_id[simp]: "aBP_get_stream_receiver_o__o⋅(aBPOut_o
   by(simp add: sbeNull.rep_eq)
 
 
-subsection ‹Identity lemmas for input SBs from streams›
+subsection \<open>Identity lemmas for input SBs from streams\<close>
 
-lemma abpin_stream_i_i__sender_i_id[simp]: "aBP_get_stream_i__sender_i⋅(aBPIn_stream_i⋅port_i__sender_port_i) = port_i__sender_port_i"
+lemma abpin_stream_i_i__sender_i_id[simp]: "aBP_get_stream_i__sender_i\<cdot>(aBPIn_stream_i\<cdot>port_i__sender_port_i) = port_i__sender_port_i"
   apply(auto simp add: aBP_get_stream_i__sender_i.rep_eq aBPIn_stream_i_def ubclUnion_ubundle_def)
   by (metis aBP_get_stream_i__sender_i.rep_eq abp_stream_i__sender_i_id)
 
 
-subsection ‹Identity lemmas for output SBs from streams›
+subsection \<open>Identity lemmas for output SBs from streams\<close>
 
-lemma abpout_stream_o_receiver_o__o_id[simp]: "aBP_get_stream_receiver_o__o⋅(aBPOut_stream_o⋅receiver_port_o__port_o) = receiver_port_o__port_o"
+lemma abpout_stream_o_receiver_o__o_id[simp]: "aBP_get_stream_receiver_o__o\<cdot>(aBPOut_stream_o\<cdot>receiver_port_o__port_o) = receiver_port_o__port_o"
   apply(auto simp add: aBP_get_stream_receiver_o__o.rep_eq aBPOut_stream_o_def ubclUnion_ubundle_def)
   by (metis aBP_get_stream_receiver_o__o.rep_eq abp_stream_receiver_o__o_id)
 
