abp/ReceiverAutomaton.thy
@@ -3,7 +3,7 @@
  * This file was generated from Receiver.maa and will be overridden when changed. To change
  * permanently, consider changing the model itself.
  *
- * Generated on Oct 2, 2018 7:11:56 PM by isartransformer 1.0.0
+ * Generated on Oct 2, 2018 7:49:38 PM by isartransformer 1.0.0
  *)
 theory ReceiverAutomaton
   imports bundle.tsynBundle automat.dAutomaton
@@ -18,7 +18,7 @@ fun prepend :: "'a::type list \<Rightarrow> 'a \<Rightarrow> 'a list" where
 
 section \<open>Datatype definition\<close>
 
-datatype ('e::countable) receiverMessage = DoNotUse_243b33898468406b9e941a9b4ac72937_ReceiverPair_E_Bool "('e\<times>bool)" | DoNotUse_243b33898468406b9e941a9b4ac72937_ReceiverBool "bool" | DoNotUse_243b33898468406b9e941a9b4ac72937_ReceiverE "'e"
+datatype ('e::countable) receiverMessage = ReceiverPair_E_Bool "('e\<times>bool)" | ReceiverBool "bool" | ReceiverE "'e"
 
 instance receiverMessage :: (countable) countable
   apply(intro_classes)
@@ -28,9 +28,9 @@ instantiation receiverMessage :: (countable) message
 begin
   fun ctype_receiverMessage :: "channel \<Rightarrow> ('e::countable) receiverMessage set" where
   "ctype_receiverMessage c = (
-    if c = \<C> ''DoNotUse_243b33898468406b9e941a9b4ac72937_dr'' then range DoNotUse_243b33898468406b9e941a9b4ac72937_ReceiverPair_E_Bool else
-    if c = \<C> ''DoNotUse_243b33898468406b9e941a9b4ac72937_ar'' then range DoNotUse_243b33898468406b9e941a9b4ac72937_ReceiverBool else
-    if c = \<C> ''DoNotUse_243b33898468406b9e941a9b4ac72937_o'' then range DoNotUse_243b33898468406b9e941a9b4ac72937_ReceiverE else
+    if c = \<C> ''dr'' then range ReceiverPair_E_Bool else
+    if c = \<C> ''ar'' then range ReceiverBool else
+    if c = \<C> ''o'' then range ReceiverE else
     undefined)"
   instance
     by(intro_classes)
@@ -40,17 +40,17 @@ end
 section \<open>Domain and range\<close>
 
 definition receiverDom :: "channel set" where
-"receiverDom = {\<C> ''DoNotUse_243b33898468406b9e941a9b4ac72937_dr''}"
+"receiverDom = {\<C> ''dr''}"
 
 definition receiverRan :: "channel set" where
-"receiverRan = {\<C> ''DoNotUse_243b33898468406b9e941a9b4ac72937_ar'', \<C> ''DoNotUse_243b33898468406b9e941a9b4ac72937_o''}"
+"receiverRan = {\<C> ''ar'', \<C> ''o''}"
 
 
 section \<open>Helpers to create a bundle from a single raw element\<close>
 
 (* Do not use this, use receiverElemIn_dr instead *)
 lift_definition receiverElem_raw_dr :: "('e\<times>bool) \<Rightarrow> ('e::countable) receiverMessage tsyn sbElem" is
-"\<lambda>x. [\<C> ''DoNotUse_243b33898468406b9e941a9b4ac72937_dr'' \<mapsto> Msg (DoNotUse_243b33898468406b9e941a9b4ac72937_ReceiverPair_E_Bool x)]"
+"\<lambda>x. [\<C> ''dr'' \<mapsto> Msg (ReceiverPair_E_Bool x)]"
   unfolding sbElemWell_def
   unfolding usclOkay_stream_def
   unfolding ctype_tsyn_def
@@ -58,7 +58,7 @@ lift_definition receiverElem_raw_dr :: "('e\<times>bool) \<Rightarrow> ('e::coun
 
 (* Do not use this, use receiverElemOut_ar_o instead *)
 lift_definition receiverElem_raw_ar :: "bool \<Rightarrow> ('e::countable) receiverMessage tsyn sbElem" is
-"\<lambda>x. [\<C> ''DoNotUse_243b33898468406b9e941a9b4ac72937_ar'' \<mapsto> Msg (DoNotUse_243b33898468406b9e941a9b4ac72937_ReceiverBool x)]"
+"\<lambda>x. [\<C> ''ar'' \<mapsto> Msg (ReceiverBool x)]"
   unfolding sbElemWell_def
   unfolding usclOkay_stream_def
   unfolding ctype_tsyn_def
@@ -66,7 +66,7 @@ lift_definition receiverElem_raw_ar :: "bool \<Rightarrow> ('e::countable) recei
 
 (* Do not use this, use receiverElemOut_ar_o instead *)
 lift_definition receiverElem_raw_o :: "'e \<Rightarrow> ('e::countable) receiverMessage tsyn sbElem" is
-"\<lambda>x. [\<C> ''DoNotUse_243b33898468406b9e941a9b4ac72937_o'' \<mapsto> Msg (DoNotUse_243b33898468406b9e941a9b4ac72937_ReceiverE x)]"
+"\<lambda>x. [\<C> ''o'' \<mapsto> Msg (ReceiverE x)]"
   unfolding sbElemWell_def
   unfolding usclOkay_stream_def
   unfolding ctype_tsyn_def
@@ -78,7 +78,7 @@ section \<open>Helpers to create a bundle from a single tsyn element\<close>
 (* Do not use this, use receiverElemIn_dr instead *)
 fun receiverElem_dr :: "('e\<times>bool) tsyn \<Rightarrow> ('e::countable) receiverMessage tsyn sbElem" where
 "receiverElem_dr (Msg port_dr) = receiverElem_raw_dr port_dr" |
-"receiverElem_dr null = sbeNull {\<C> ''DoNotUse_243b33898468406b9e941a9b4ac72937_dr''}"
+"receiverElem_dr null = sbeNull {\<C> ''dr''}"
 
 declare receiverElem_dr.simps[simp del]
 
@@ -89,7 +89,7 @@ definition receiver_dr :: "('e\<times>bool) tsyn \<Rightarrow> ('e::countable) r
 (* Do not use this, use receiverElemOut_ar_o instead *)
 fun receiverElem_ar :: "bool tsyn \<Rightarrow> ('e::countable) receiverMessage tsyn sbElem" where
 "receiverElem_ar (Msg port_ar) = receiverElem_raw_ar port_ar" |
-"receiverElem_ar null = sbeNull {\<C> ''DoNotUse_243b33898468406b9e941a9b4ac72937_ar''}"
+"receiverElem_ar null = sbeNull {\<C> ''ar''}"
 
 declare receiverElem_ar.simps[simp del]
 
@@ -100,7 +100,7 @@ definition receiver_ar :: "bool tsyn \<Rightarrow> ('e::countable) receiverMessa
 (* Do not use this, use receiverElemOut_ar_o instead *)
 fun receiverElem_o :: "'e tsyn \<Rightarrow> ('e::countable) receiverMessage tsyn sbElem" where
 "receiverElem_o (Msg port_o) = receiverElem_raw_o port_o" |
-"receiverElem_o null = sbeNull {\<C> ''DoNotUse_243b33898468406b9e941a9b4ac72937_o''}"
+"receiverElem_o null = sbeNull {\<C> ''o''}"
 
 declare receiverElem_o.simps[simp del]
 
@@ -130,21 +130,21 @@ section \<open>Helpers to create a bundle from a tsyn list of elements\<close>
 (* Do not use this, use receiverIn_list_dr instead *)
 fun receiver_list_dr :: "(('e\<times>bool) tsyn) list \<Rightarrow> ('e::countable) receiverMessage tsyn SB" where
 "receiver_list_dr (x#xs) = ubConcEq (receiver_dr x)\<cdot>(receiver_list_dr xs)" |
-"receiver_list_dr []     = ubLeast {\<C> ''DoNotUse_243b33898468406b9e941a9b4ac72937_dr''}"
+"receiver_list_dr []     = ubLeast {\<C> ''dr''}"
 
 declare receiver_list_dr.simps[simp del]
 
 (* Do not use this, use receiverOut_list_ar_o instead *)
 fun receiver_list_ar :: "(bool tsyn) list \<Rightarrow> ('e::countable) receiverMessage tsyn SB" where
 "receiver_list_ar (x#xs) = ubConcEq (receiver_ar x)\<cdot>(receiver_list_ar xs)" |
-"receiver_list_ar []     = ubLeast {\<C> ''DoNotUse_243b33898468406b9e941a9b4ac72937_ar''}"
+"receiver_list_ar []     = ubLeast {\<C> ''ar''}"
 
 declare receiver_list_ar.simps[simp del]
 
 (* Do not use this, use receiverOut_list_ar_o instead *)
 fun receiver_list_o :: "('e tsyn) list \<Rightarrow> ('e::countable) receiverMessage tsyn SB" where
 "receiver_list_o (x#xs) = ubConcEq (receiver_o x)\<cdot>(receiver_list_o xs)" |
-"receiver_list_o []     = ubLeast {\<C> ''DoNotUse_243b33898468406b9e941a9b4ac72937_o''}"
+"receiver_list_o []     = ubLeast {\<C> ''o''}"
 
 declare receiver_list_o.simps[simp del]
 
@@ -161,44 +161,44 @@ fun receiverOut_list_ar_o :: "(bool tsyn\<times>'e tsyn) list \<Rightarrow> ('e:
 
 section \<open>Helpers to create a bundle from a tsyn stream of elements\<close>
 
-lift_definition DoNotUse_243b33898468406b9e941a9b4ac72937_receiver_stream_dr_h :: "('e\<times>bool) tsyn stream \<Rightarrow> ('e::countable) receiverMessage tsyn SB" is
-"\<lambda> s. [(\<C> ''DoNotUse_243b33898468406b9e941a9b4ac72937_dr'') \<mapsto> (tsynMap (DoNotUse_243b33898468406b9e941a9b4ac72937_ReceiverPair_E_Bool)\<cdot>s)]"
+lift_definition receiver_stream_dr_h :: "('e\<times>bool) tsyn stream \<Rightarrow> ('e::countable) receiverMessage tsyn SB" is
+"\<lambda> s. [(\<C> ''dr'') \<mapsto> (tsynMap (ReceiverPair_E_Bool)\<cdot>s)]"
   unfolding ubWell_def usclOkay_stream_def ctype_tsyn_def
   by auto
 
 (* Do not use this, use receiverIn_stream_dr instead *)
 lift_definition receiver_stream_dr :: "(('e\<times>bool)) tsyn stream \<rightarrow> ('e::countable) receiverMessage tsyn SB" is
-"DoNotUse_243b33898468406b9e941a9b4ac72937_receiver_stream_dr_h"
-  apply(auto simp add: cfun_def DoNotUse_243b33898468406b9e941a9b4ac72937_receiver_stream_dr_h_def map_fun_def comp_def)
+"receiver_stream_dr_h"
+  apply(auto simp add: cfun_def receiver_stream_dr_h_def map_fun_def comp_def)
   apply(rule cont_Abs_UB)
   apply(simp add: option_one_cont)
-  by (metis DoNotUse_243b33898468406b9e941a9b4ac72937_receiver_stream_dr_h.rep_eq ubrep_well)
+  by (metis receiver_stream_dr_h.rep_eq ubrep_well)
 
-lift_definition DoNotUse_243b33898468406b9e941a9b4ac72937_receiver_stream_ar_h :: "bool tsyn stream \<Rightarrow> ('e::countable) receiverMessage tsyn SB" is
-"\<lambda> s. [(\<C> ''DoNotUse_243b33898468406b9e941a9b4ac72937_ar'') \<mapsto> (tsynMap (DoNotUse_243b33898468406b9e941a9b4ac72937_ReceiverBool)\<cdot>s)]"
+lift_definition receiver_stream_ar_h :: "bool tsyn stream \<Rightarrow> ('e::countable) receiverMessage tsyn SB" is
+"\<lambda> s. [(\<C> ''ar'') \<mapsto> (tsynMap (ReceiverBool)\<cdot>s)]"
   unfolding ubWell_def usclOkay_stream_def ctype_tsyn_def
   by auto
 
 (* Do not use this, use receiverOut_stream_ar_o instead *)
 lift_definition receiver_stream_ar :: "(bool) tsyn stream \<rightarrow> ('e::countable) receiverMessage tsyn SB" is
-"DoNotUse_243b33898468406b9e941a9b4ac72937_receiver_stream_ar_h"
-  apply(auto simp add: cfun_def DoNotUse_243b33898468406b9e941a9b4ac72937_receiver_stream_ar_h_def map_fun_def comp_def)
+"receiver_stream_ar_h"
+  apply(auto simp add: cfun_def receiver_stream_ar_h_def map_fun_def comp_def)
   apply(rule cont_Abs_UB)
   apply(simp add: option_one_cont)
-  by (metis DoNotUse_243b33898468406b9e941a9b4ac72937_receiver_stream_ar_h.rep_eq ubrep_well)
+  by (metis receiver_stream_ar_h.rep_eq ubrep_well)
 
-lift_definition DoNotUse_243b33898468406b9e941a9b4ac72937_receiver_stream_o_h :: "'e tsyn stream \<Rightarrow> ('e::countable) receiverMessage tsyn SB" is
-"\<lambda> s. [(\<C> ''DoNotUse_243b33898468406b9e941a9b4ac72937_o'') \<mapsto> (tsynMap (DoNotUse_243b33898468406b9e941a9b4ac72937_ReceiverE)\<cdot>s)]"
+lift_definition receiver_stream_o_h :: "'e tsyn stream \<Rightarrow> ('e::countable) receiverMessage tsyn SB" is
+"\<lambda> s. [(\<C> ''o'') \<mapsto> (tsynMap (ReceiverE)\<cdot>s)]"
   unfolding ubWell_def usclOkay_stream_def ctype_tsyn_def
   by auto
 
 (* Do not use this, use receiverOut_stream_ar_o instead *)
 lift_definition receiver_stream_o :: "('e) tsyn stream \<rightarrow> ('e::countable) receiverMessage tsyn SB" is
-"DoNotUse_243b33898468406b9e941a9b4ac72937_receiver_stream_o_h"
-  apply(auto simp add: cfun_def DoNotUse_243b33898468406b9e941a9b4ac72937_receiver_stream_o_h_def map_fun_def comp_def)
+"receiver_stream_o_h"
+  apply(auto simp add: cfun_def receiver_stream_o_h_def map_fun_def comp_def)
   apply(rule cont_Abs_UB)
   apply(simp add: option_one_cont)
-  by (metis DoNotUse_243b33898468406b9e941a9b4ac72937_receiver_stream_o_h.rep_eq ubrep_well)
+  by (metis receiver_stream_o_h.rep_eq ubrep_well)
 
 (* Create one SB for all input channels *)
 definition receiverIn_stream_dr :: "('e\<times>bool) tsyn stream \<rightarrow> ('e::countable) receiverMessage tsyn SB" where
@@ -212,24 +212,24 @@ definition receiverOut_stream_ar_o :: "bool tsyn stream \<rightarrow> 'e tsyn st
 section \<open>Helpers to get tsyn elements and streams from sbElems and SBs\<close>
 
 definition receiverElem_get_dr :: "('e::countable) receiverMessage tsyn sbElem \<Rightarrow> (('e\<times>bool)) tsyn" where
-"receiverElem_get_dr sbe = tsynApplyElem (inv DoNotUse_243b33898468406b9e941a9b4ac72937_ReceiverPair_E_Bool) ((Rep_sbElem sbe) \<rightharpoonup> (\<C> ''DoNotUse_243b33898468406b9e941a9b4ac72937_dr''))"
+"receiverElem_get_dr sbe = tsynApplyElem (inv ReceiverPair_E_Bool) ((Rep_sbElem sbe) \<rightharpoonup> (\<C> ''dr''))"
 
 lift_definition receiver_get_stream_dr :: "('e::countable) receiverMessage tsyn SB \<rightarrow> ('e\<times>bool) tsyn stream" is
-"\<lambda>sb. tsynMap (inv DoNotUse_243b33898468406b9e941a9b4ac72937_ReceiverPair_E_Bool)\<cdot>(sb . (\<C> ''DoNotUse_243b33898468406b9e941a9b4ac72937_dr''))"
+"\<lambda>sb. tsynMap (inv ReceiverPair_E_Bool)\<cdot>(sb . (\<C> ''dr''))"
   by(simp add: cfun_def)
 
 definition receiverElem_get_ar :: "('e::countable) receiverMessage tsyn sbElem \<Rightarrow> (bool) tsyn" where
-"receiverElem_get_ar sbe = tsynApplyElem (inv DoNotUse_243b33898468406b9e941a9b4ac72937_ReceiverBool) ((Rep_sbElem sbe) \<rightharpoonup> (\<C> ''DoNotUse_243b33898468406b9e941a9b4ac72937_ar''))"
+"receiverElem_get_ar sbe = tsynApplyElem (inv ReceiverBool) ((Rep_sbElem sbe) \<rightharpoonup> (\<C> ''ar''))"
 
 lift_definition receiver_get_stream_ar :: "('e::countable) receiverMessage tsyn SB \<rightarrow> bool tsyn stream" is
-"\<lambda>sb. tsynMap (inv DoNotUse_243b33898468406b9e941a9b4ac72937_ReceiverBool)\<cdot>(sb . (\<C> ''DoNotUse_243b33898468406b9e941a9b4ac72937_ar''))"
+"\<lambda>sb. tsynMap (inv ReceiverBool)\<cdot>(sb . (\<C> ''ar''))"
   by(simp add: cfun_def)
 
 definition receiverElem_get_o :: "('e::countable) receiverMessage tsyn sbElem \<Rightarrow> ('e) tsyn" where
-"receiverElem_get_o sbe = tsynApplyElem (inv DoNotUse_243b33898468406b9e941a9b4ac72937_ReceiverE) ((Rep_sbElem sbe) \<rightharpoonup> (\<C> ''DoNotUse_243b33898468406b9e941a9b4ac72937_o''))"
+"receiverElem_get_o sbe = tsynApplyElem (inv ReceiverE) ((Rep_sbElem sbe) \<rightharpoonup> (\<C> ''o''))"
 
 lift_definition receiver_get_stream_o :: "('e::countable) receiverMessage tsyn SB \<rightarrow> 'e tsyn stream" is
-"\<lambda>sb. tsynMap (inv DoNotUse_243b33898468406b9e941a9b4ac72937_ReceiverE)\<cdot>(sb . (\<C> ''DoNotUse_243b33898468406b9e941a9b4ac72937_o''))"
+"\<lambda>sb. tsynMap (inv ReceiverE)\<cdot>(sb . (\<C> ''o''))"
   by(simp add: cfun_def)
 
 
@@ -314,17 +314,17 @@ lemma receiverautomaton_ran[simp]: "daRan receiverAutomaton = receiverRan"
 
 section \<open>Lemmas for single tsyn setter\<close>
 
-lemma receiverelem_dr_dom[simp]: "sbeDom (receiverElem_dr x) = {\<C> ''DoNotUse_243b33898468406b9e941a9b4ac72937_dr''}"
+lemma receiverelem_dr_dom[simp]: "sbeDom (receiverElem_dr x) = {\<C> ''dr''}"
   apply(cases x)
   apply(simp add: receiverElem_dr.simps sbeDom_def receiverElem_raw_dr.rep_eq)
   by(simp add: receiverElem_dr.simps)
 
-lemma receiverelem_ar_dom[simp]: "sbeDom (receiverElem_ar x) = {\<C> ''DoNotUse_243b33898468406b9e941a9b4ac72937_ar''}"
+lemma receiverelem_ar_dom[simp]: "sbeDom (receiverElem_ar x) = {\<C> ''ar''}"
   apply(cases x)
   apply(simp add: receiverElem_ar.simps sbeDom_def receiverElem_raw_ar.rep_eq)
   by(simp add: receiverElem_ar.simps)
 
-lemma receiverelem_o_dom[simp]: "sbeDom (receiverElem_o x) = {\<C> ''DoNotUse_243b33898468406b9e941a9b4ac72937_o''}"
+lemma receiverelem_o_dom[simp]: "sbeDom (receiverElem_o x) = {\<C> ''o''}"
   apply(cases x)
   apply(simp add: receiverElem_o.simps sbeDom_def receiverElem_raw_o.rep_eq)
   by(simp add: receiverElem_o.simps)
@@ -342,23 +342,25 @@ lemma receiverout_ar_o_dom[simp]: "ubDom\<cdot>(receiverOut_ar_o port_ar port_o)
   by(simp add: receiverOut_ar_o_def)
 
 
-section \<open>stream-setter (just for simp)\<close>
+section \<open>Stream-setter\<close>
 
-(* SWS: Allen Lemma einen Namen geben *)
-lemma [simp]: "ubDom\<cdot>(receiver_stream_dr\<cdot>x) = {\<C> ''DoNotUse_243b33898468406b9e941a9b4ac72937_dr''}"
-  by(simp add: receiver_stream_dr.rep_eq ubdom_insert DoNotUse_243b33898468406b9e941a9b4ac72937_receiver_stream_dr_h.rep_eq)
+lemma receiver_stream_dr_dom[simp]: "ubDom\<cdot>(receiver_stream_dr\<cdot>x) = {\<C> ''dr''}"
+  by(simp add: receiver_stream_dr.rep_eq ubdom_insert receiver_stream_dr_h.rep_eq)
 
-lemma [simp]: "ubDom\<cdot>(receiver_stream_ar\<cdot>x) = {\<C> ''DoNotUse_243b33898468406b9e941a9b4ac72937_ar''}"
-  by(simp add: receiver_stream_ar.rep_eq ubdom_insert DoNotUse_243b33898468406b9e941a9b4ac72937_receiver_stream_ar_h.rep_eq)
+lemma receiver_stream_ar_dom[simp]: "ubDom\<cdot>(receiver_stream_ar\<cdot>x) = {\<C> ''ar''}"
+  by(simp add: receiver_stream_ar.rep_eq ubdom_insert receiver_stream_ar_h.rep_eq)
 
-lemma [simp]: "ubDom\<cdot>(receiver_stream_o\<cdot>x) = {\<C> ''DoNotUse_243b33898468406b9e941a9b4ac72937_o''}"
-  by(simp add: receiver_stream_o.rep_eq ubdom_insert DoNotUse_243b33898468406b9e941a9b4ac72937_receiver_stream_o_h.rep_eq)
+lemma receiver_stream_o_dom[simp]: "ubDom\<cdot>(receiver_stream_o\<cdot>x) = {\<C> ''o''}"
+  by(simp add: receiver_stream_o.rep_eq ubdom_insert receiver_stream_o_h.rep_eq)
 
-(* SWS: Analog für In *)
-lemma [simp]: "ubDom\<cdot>(receiverOut_stream_ar_o\<cdot>port_ar\<cdot>port_o) = receiverRan"
-  apply(simp add: receiverOut_stream_ar_o_def)
-  apply(simp add: ubclUnion_ubundle_def)
+lemma receiverin_stream_dr_dom[simp]: "ubDom\<cdot>(receiverIn_stream_dr\<cdot>port_dr) = receiverDom"
+  apply(simp add: receiverIn_stream_dr_def ubclUnion_ubundle_def)
+  by(auto simp add: receiverDom_def)
+
+lemma receiverout_stream_ar_o_dom[simp]: "ubDom\<cdot>(receiverOut_stream_ar_o\<cdot>port_ar\<cdot>port_o) = receiverRan"
+  apply(simp add: receiverOut_stream_ar_o_def ubclUnion_ubundle_def)
   by(auto simp add: receiverRan_def)
+
 
 section \<open>Lemmas for getter\<close>
 
@@ -393,17 +395,17 @@ subsection \<open>Identity lemmas for single SBs from streams\<close>
 
 lemma receiver_stream_dr_id[simp]: "receiver_get_stream_dr\<cdot>(receiver_stream_dr\<cdot>x) = x"
   apply(simp add: receiver_get_stream_dr.rep_eq receiver_stream_dr.rep_eq)
-  apply(simp add: ubGetCh_def DoNotUse_243b33898468406b9e941a9b4ac72937_receiver_stream_dr_h.rep_eq)
+  apply(simp add: ubGetCh_def receiver_stream_dr_h.rep_eq)
   by (simp add: inj_def)
 
 lemma receiver_stream_ar_id[simp]: "receiver_get_stream_ar\<cdot>(receiver_stream_ar\<cdot>x) = x"
   apply(simp add: receiver_get_stream_ar.rep_eq receiver_stream_ar.rep_eq)
-  apply(simp add: ubGetCh_def DoNotUse_243b33898468406b9e941a9b4ac72937_receiver_stream_ar_h.rep_eq)
+  apply(simp add: ubGetCh_def receiver_stream_ar_h.rep_eq)
   by (simp add: inj_def)
 
 lemma receiver_stream_o_id[simp]: "receiver_get_stream_o\<cdot>(receiver_stream_o\<cdot>x) = x"
   apply(simp add: receiver_get_stream_o.rep_eq receiver_stream_o.rep_eq)
-  apply(simp add: ubGetCh_def DoNotUse_243b33898468406b9e941a9b4ac72937_receiver_stream_o_h.rep_eq)
+  apply(simp add: ubGetCh_def receiver_stream_o_h.rep_eq)
   by (simp add: inj_def)
 
 
